Adjusted assign costs
Adjusted assign costs to only depend on assigned arithmetic expression.
Skip costs probably need the same adjustment.

IMP-/Step_Semantics_Cost_Generalization/Big_StepT_Ex_GC_Final.thy
@@ -1,25 +1,25 @@
 
-theory Big_StepT_Ex_GC
-  imports Big_StepT_Generalized_Cost "~~/src/HOL/Library/Simps_Case_Conv"
+theory Big_StepT_Ex_GC_Final
+  imports Big_StepT_Generalized_Cost_Final "~~/src/HOL/Library/Simps_Case_Conv"
 begin
                   
 context BS_Generalized_Cost begin      
 
-function (sequential, domintros) big_step_function :: "(com \<times> state) \<Rightarrow> (('a \<Rightarrow> nat) \<times> state)" where
-  "big_step_function (SKIP,s) = (skip_costs, s)" |
-  "big_step_function (x ::= a,s) = (assign_costs, s(x := aval a s))" |
+function (sequential, domintros) big_step_function :: "(com \<times> state) \<Rightarrow> (nat \<times> state)" where
+  "big_step_function (SKIP,s) = (skip_costs s, s)" |
+  "big_step_function (x ::= a,s) = (assign_costs a s, s(x := aval a s))" |
   "big_step_function (c1;;c2, s) =
     (let (n1, s1) = big_step_function (c1, s);
         (n2, s2) = big_step_function (c2, s1)
-    in (Plus_lifted n1 n2, s2))" |
+    in (n1 + n2, s2))" |
   "big_step_function (IF b \<noteq>0 THEN c1 ELSE c2, s) = 
-    apfst Suc_lifted (if s b \<noteq> 0 then big_step_function (c1,s) else big_step_function (c2,s))" |
-  "big_step_function (WHILE b \<noteq>0 DO c,s) = (if s b \<noteq> 0 then apfst Suc_lifted (big_step_function (c;; WHILE b \<noteq>0 DO c, s)) else (while_exit_costs, s))" 
+    apfst Suc (if s b \<noteq> 0 then big_step_function (c1,s) else big_step_function (c2,s))" |
+  "big_step_function (WHILE b \<noteq>0 DO c,s) = (if s b \<noteq> 0 then apfst Suc (big_step_function (c;; WHILE b \<noteq>0 DO c, s)) else (while_exit_costs s, s))" 
   by pat_completeness auto
 
 print_theorems
 (* Soundness and partial termination *)
-lemma "(c,s) \<Rightarrow>\<^bsup>t\<^esup> s' \<Longrightarrow> big_step_function_dom (c,s) \<and> big_step_function (c,s) = (t, s')"
+lemma "(c,s) \<Rightarrow>\<^sub>G\<^bsup> t \<^esup> s' \<Longrightarrow> big_step_function_dom (c,s) \<and> big_step_function (c,s) = (t, s')"
 proof (induction  rule: big_step_tG.induct)
   case (Skip s)
   then show ?case 
@@ -32,16 +32,13 @@ next
   case (Seq c1 s1 C1 s2 c2 C2 s3 C3)
   then show ?case 
       apply (subst big_step_function.psimps)
-     apply (auto intro: big_step_function.domintros simp add: Let_def big_step_function.domintros big_step_function.psimps)
-    by (simp add: Plus_lifted_def) (* ? ? ? *)
+    by (auto intro: big_step_function.domintros simp add: Let_def big_step_function.domintros big_step_function.psimps) (* ? ? ? *)
 next
   case (IfTrue s b c1 C t C' c2)
-  then show ?case apply (auto intro: big_step_function.domintros simp add: Let_def big_step_function.domintros big_step_function.psimps)
-    by (simp add: Suc_lifted_def)
+  then show ?case by (auto intro: big_step_function.domintros simp add: Let_def big_step_function.domintros big_step_function.psimps)
 next
   case (IfFalse s b c2 C t C' c1)
-  then show ?case apply (auto intro: big_step_function.domintros simp add: Let_def big_step_function.domintros big_step_function.psimps)
-    by (simp add: Suc_lifted_def)
+  then show ?case by (auto intro: big_step_function.domintros simp add: Let_def big_step_function.domintros big_step_function.psimps)
 next
   case (WhileFalse s b c)
    then show ?case by (auto intro: big_step_function.domintros simp add: Let_def big_step_function.domintros big_step_function.psimps)
@@ -60,10 +57,7 @@ next
     apply (simp add: WhileTrue.IH(1) WhileTrue.IH(2))
       apply (unfold Let_def)
     using WhileTrue.IH(1) WhileTrue.IH(2) WhileTrue.hyps(4) 
-      apply (auto split: prod.splits)[]
-      apply (simp add: Plus_lifted_def Suc_lifted_def)
-     apply (simp add: WhileTrue.hyps(1))
-    by (simp add: WhileTrue.hyps(1))
+    by (simp add: WhileTrue.hyps(1))+
 qed
  (* TODO: Do properly *)
 
@@ -76,61 +70,61 @@ qed
 
 
 lemma mono1[partial_function_mono]: "monotone option.le_fun option_ord
-          (\<lambda>big_step_ex. map_option (apfst ((Plus_lifted) aa)) (big_step_ex (x32, ba)))" 
+          (\<lambda>big_step_ex. map_option (apfst ((+) aa)) (big_step_ex (x32, ba)))" 
   by (smt (verit, best) flat_ord_def fun_ord_def monotoneI option.map_disc_iff)
-lemma "monotone option.le_fun option_ord
+lemma mono4[partial_function_mono]:"monotone option.le_fun option_ord
           (\<lambda>big_step_ex.
-              map_option (apfst Suc_lifted)
+              map_option (apfst Suc)
                (if b x41 \<noteq> 0 then big_step_ex (x42, b) else big_step_ex (x43, b)))"
   by (smt (verit, best) flat_ord_def fun_ord_def monotoneI option.map_disc_iff)
 lemma mono2[partial_function_mono]:"
          monotone option.le_fun option_ord
-          (\<lambda>f. map_option (apfst Suc_lifted) (f (x52;; WHILE x51\<noteq>0 DO x52, b)))"
+          (\<lambda>f. map_option (apfst Suc) (f (x52;; WHILE x51\<noteq>0 DO x52, b)))"
   by (smt (verit, best) flat_ord_def fun_ord_def monotoneI option.map_disc_iff)
 lemma mono3[partial_function_mono]:"
   (\<And>x a b x41 x42 x43.
       monotone option.le_fun option_ord
        (\<lambda>big_step_ex.
-           map_option (apfst Suc_lifted)
+           map_option (apfst Suc)
             (if b x41 \<noteq> 0 then big_step_ex (x42, b) else big_step_ex (x43, b)))) \<Longrightarrow>
   (\<And>x a b x51 x52.
       monotone option.le_fun option_ord
-       (\<lambda>f. map_option (apfst Suc_lifted) (f (x52;; WHILE x51\<noteq>0 DO x52, b)))) \<Longrightarrow>
+       (\<lambda>f. map_option (apfst Suc) (f (x52;; WHILE x51\<noteq>0 DO x52, b)))) \<Longrightarrow>
   (\<And>x. monotone option.le_fun option_ord
          (\<lambda>big_step_ex.
-             case x of (SKIP, s) \<Rightarrow> Some (skip_costs, s) | (x ::= a, s) \<Rightarrow> Some (assign_costs, s(x := aval a s))
+             case x of (SKIP, s) \<Rightarrow> Some (skip_costs s, s) | (x ::= a, s) \<Rightarrow> Some (assign_costs a s, s(x := aval a s))
              | (c1;; c2, s) \<Rightarrow>
                  Option.bind (big_step_ex (c1, s))
-                  (\<lambda>(n, s). map_option (apfst ((Plus_lifted) n)) (big_step_ex (c2, s)))
+                  (\<lambda>(n, s). map_option (apfst ((+) n)) (big_step_ex (c2, s)))
              | (IF b\<noteq>0 THEN c1 ELSE c2, s) \<Rightarrow>
-                 map_option (apfst Suc_lifted)
+                 map_option (apfst Suc)
                   (if s b \<noteq> 0 then big_step_ex (c1, s) else big_step_ex (c2, s))
              | (WHILE b\<noteq>0 DO c, s) \<Rightarrow>
-                 if s b \<noteq> 0 then map_option (apfst Suc_lifted) (big_step_ex (c;; WHILE b\<noteq>0 DO c, s))
-                 else Some (while_exit_costs, s)))"
+                 if s b \<noteq> 0 then map_option (apfst Suc) (big_step_ex (c;; WHILE b\<noteq>0 DO c, s))
+                 else Some (while_exit_costs s, s)))"
   apply (auto split: prod.splits com.splits option.splits simp add: flat_ord_def fun_ord_def monotone_def)
   apply (smt (verit) bind.bind_lunit bind_eq_None_conv old.prod.case option.collapse option.map_disc_iff split_cong)
   apply (smt (verit) bind.bind_lunit bind_eq_None_conv old.prod.case option.collapse option.map_disc_iff split_cong)
   apply (smt (verit) bind.bind_lunit bind_eq_None_conv old.prod.case option.collapse option.map_disc_iff split_cong)
   apply (smt (verit) bind.bind_lunit bind_eq_None_conv old.prod.case option.collapse option.map_disc_iff split_cong)
   done
-lemma mono4[partial_function_mono]: "monotone option.le_fun option_ord
+lemma mono5[partial_function_mono]: "monotone option.le_fun option_ord
           (\<lambda>big_step_ex.
               map_option (apfst Suc_lifted)
                (if b x41 \<noteq> 0 then big_step_ex (x42, b) else big_step_ex (x43, b)))"
   by (smt (verit, best) flat_ord_def fun_ord_def monotoneI option.map_disc_iff)
 
-partial_function (option) big_step_ex :: "(com\<times> state) \<Rightarrow> (('a \<Rightarrow> nat) \<times> state) option" where
-  "big_step_ex cs = (case cs of (SKIP,s) \<Rightarrow> Some (skip_costs, s) | (x ::= a,s) \<Rightarrow> Some (assign_costs, s(x := aval a s))
-    | (c1;;c2, s1) \<Rightarrow> Option.bind (big_step_ex (c1,s1)) (\<lambda>(n, s). map_option (apfst (\<lambda>n'. Plus_lifted n n')) (big_step_ex (c2, s)))
-    | (IF b \<noteq>0 THEN c1 ELSE c2, s) \<Rightarrow> map_option (apfst Suc_lifted) (if s b \<noteq> 0 then big_step_ex (c1,s) else big_step_ex (c2,s))
-    | (WHILE b \<noteq>0 DO c,s) \<Rightarrow> (if s b \<noteq> 0 then map_option (apfst Suc_lifted) (big_step_ex (c;; WHILE b \<noteq>0 DO c, s)) else Some (while_exit_costs, s)))"
+partial_function (option) big_step_ex :: "(com\<times> state) \<Rightarrow> (nat \<times> state) option" where
+  "big_step_ex cs = (case cs of (SKIP,s) \<Rightarrow> Some (skip_costs s, s) | (x ::= a,s) \<Rightarrow> Some (assign_costs a s, s(x := aval a s))
+    | (c1;;c2, s1) \<Rightarrow> Option.bind (big_step_ex (c1,s1)) (\<lambda>(n, s). map_option (apfst (\<lambda>n'. n+n')) (big_step_ex (c2, s)))
+    | (IF b \<noteq>0 THEN c1 ELSE c2, s) \<Rightarrow> map_option (apfst Suc) (if s b \<noteq> 0 then big_step_ex (c1,s) else big_step_ex (c2,s))
+    | (WHILE b \<noteq>0 DO c,s) \<Rightarrow> (if s b \<noteq> 0 then map_option (apfst Suc) (big_step_ex (c;; WHILE b \<noteq>0 DO c, s)) else Some (while_exit_costs s, s)))"
     
 thm big_step_ex.simps
 simps_of_case big_step_ex_simps[simp,code]: big_step_ex.simps
 
-lemma big_step_ex_sound:"(c,s) \<Rightarrow>\<^bsup>t\<^esup> s' \<Longrightarrow> big_step_ex (c,s) = Some (t, s')"
-  by (induction rule: big_step_tG.induct) (auto simp add: Suc_lifted_def Plus_lifted_def)
+lemma big_step_ex_sound:"(c,s) \<Rightarrow>\<^sub>G\<^bsup>t\<^esup> s' \<Longrightarrow> big_step_ex (c,s) = Some (t, s')"
+  by (induction rule: big_step_tG.induct) (auto)
 
 end
 end
