IMP-/Step_Semantics_Cost_Generalization/Big_StepT_Generalized_Cost.thy
@@ -1,6 +1,6 @@
 section "Big step semantics of IMP- generalized to include arbitrary* 
          command cost functions"
-theory Big_StepT_Generalized_Cost imports "../Max_Constant" Main  "../Com" "HOL-Eisbach.Eisbach_Tools" begin
+theory Big_StepT_Generalized_Cost imports "../Max_Constant" Main "../Nat_Dom_Lifted" "../Com" "HOL-Eisbach.Eisbach_Tools" begin
 
 paragraph "Summary"
 text\<open>We attempt to generalize big step semantics with time for IMP-. 
@@ -11,32 +11,35 @@ subsection "Big step semantics definition:"
 text "In IMP- Branching is only based on whether a variable's value equals 0."
 
 locale BS_Generalized_Cost =
-  fixes skip_costs :: "'a \<Rightarrow> nat" and 
-      assign_costs :: "'a \<Rightarrow> nat"
-    assumes assign_cost_positive: "\<forall>x. assign_costs x > 0"
+  fixes skip_costs :: "state \<Rightarrow> nat" and 
+      assign_costs :: "aexp \<Rightarrow> state \<Rightarrow> nat"
+    assumes skip_cost_least: "\<And>x s s'. skip_costs s \<le> assign_costs x s'"
+    assumes assign_cost_positive: "\<And>x s. assign_costs x s > 0"
 begin 
 
+abbreviation "while_exit_costs \<equiv> (\<lambda>x. 2 * (skip_costs x))"
+
 inductive
-  big_step_tG :: "com \<times> state \<Rightarrow> ('a \<Rightarrow> nat) \<Rightarrow> state \<Rightarrow> bool"  ("_ \<Rightarrow>\<^bsup> _ \<^esup> _" 55)
+  big_step_tG :: "com \<times> state \<Rightarrow> ('a \<Rightarrow> nat) \<Rightarrow> state \<Rightarrow> bool"  ("_ \<Rightarrow>\<^sub>G\<^bsup> _ \<^esup> _" 55)
 where
-Skip: "(SKIP,s) \<Rightarrow>\<^bsup> skip_costs \<^esup> s"|
-Assign: "(x ::= a,s) \<Rightarrow>\<^bsup> assign_costs \<^esup> s(x := aval a s)" |
-Seq: "\<lbrakk> (c1,s1) \<Rightarrow>\<^bsup> C1 \<^esup> s2;  (c2,s2) \<Rightarrow>\<^bsup> C2 \<^esup> s3 ; C3 = (\<lambda>x. (C1 x) + (C2 x)) \<rbrakk> \<Longrightarrow> (c1;;c2, s1) \<Rightarrow>\<^bsup> C3 \<^esup> s3" |
-IfTrue: "\<lbrakk> s b \<noteq> 0;  (c1,s) \<Rightarrow>\<^bsup> C \<^esup> t; C'= (\<lambda>x. (C x) + 1) \<rbrakk> \<Longrightarrow> (IF b \<noteq>0 THEN c1 ELSE c2, s) \<Rightarrow>\<^bsup> C' \<^esup> t" |
-IfFalse: "\<lbrakk> s b = 0; (c2,s) \<Rightarrow>\<^bsup> C \<^esup> t; C'= (\<lambda>x. (C x) + 1)  \<rbrakk> \<Longrightarrow> (IF b \<noteq>0 THEN c1 ELSE c2, s) \<Rightarrow>\<^bsup> C' \<^esup> t" |
-WhileFalse: "\<lbrakk> s b = 0 \<rbrakk> \<Longrightarrow> (WHILE b \<noteq>0 DO c,s) \<Rightarrow>\<^bsup> (\<lambda>x. 2 * (skip_costs x)) \<^esup> s" |
-WhileTrue: "\<lbrakk> s1 b \<noteq> 0;  (c,s1) \<Rightarrow>\<^bsup> C1 \<^esup> s2;  (WHILE b \<noteq>0 DO c, s2) \<Rightarrow>\<^bsup> C2 \<^esup> s3; C3 = (\<lambda>x. (C1 x) + (C2 x) + 1)\<rbrakk> 
-    \<Longrightarrow> (WHILE b \<noteq>0 DO c, s1) \<Rightarrow>\<^bsup> C3 \<^esup> s3" 
+Skip: "(SKIP,s) \<Rightarrow>\<^sub>G\<^bsup> skip_costs \<^esup> s"|
+Assign: "(x ::= a,s) \<Rightarrow>\<^sub>G\<^bsup> assign_costs \<^esup> s(x := aval a s)" |
+Seq: "\<lbrakk> (c1,s1) \<Rightarrow>\<^sub>G\<^bsup> C1 \<^esup> s2;  (c2,s2) \<Rightarrow>\<^sub>G\<^bsup> C2 \<^esup> s3 ; C3 = (\<lambda>x. (C1 x) + (C2 x)) \<rbrakk> \<Longrightarrow> (c1;;c2, s1) \<Rightarrow>\<^sub>G\<^bsup> C3 \<^esup> s3" |
+IfTrue: "\<lbrakk> s b \<noteq> 0;  (c1,s) \<Rightarrow>\<^sub>G\<^bsup> C \<^esup> t; C'= (\<lambda>x. (C x) + 1) \<rbrakk> \<Longrightarrow> (IF b \<noteq>0 THEN c1 ELSE c2, s) \<Rightarrow>\<^sub>G\<^bsup> C' \<^esup> t" |
+IfFalse: "\<lbrakk> s b = 0; (c2,s) \<Rightarrow>\<^sub>G\<^bsup> C \<^esup> t; C'= (\<lambda>x. (C x) + 1)  \<rbrakk> \<Longrightarrow> (IF b \<noteq>0 THEN c1 ELSE c2, s) \<Rightarrow>\<^sub>G\<^bsup> C' \<^esup> t" |
+WhileFalse: "\<lbrakk> s b = 0 \<rbrakk> \<Longrightarrow> (WHILE b \<noteq>0 DO c,s) \<Rightarrow>\<^sub>G\<^bsup> (\<lambda>x. 2 * (skip_costs x)) \<^esup> s" |
+WhileTrue: "\<lbrakk> s1 b \<noteq> 0;  (c,s1) \<Rightarrow>\<^sub>G\<^bsup> C1 \<^esup> s2;  (WHILE b \<noteq>0 DO c, s2) \<Rightarrow>\<^sub>G\<^bsup> C2 \<^esup> s3; C3 = (\<lambda>x. (C1 x) + (C2 x) + 1)\<rbrakk> 
+    \<Longrightarrow> (WHILE b \<noteq>0 DO c, s1) \<Rightarrow>\<^sub>G\<^bsup> C3 \<^esup> s3" 
 end
 
 bundle big_stepG_syntax
 begin
-notation BS_Generalized_Cost.big_step_tG ("_ \<Rightarrow>\<^bsup> _ \<^esup> _" 55)
+notation BS_Generalized_Cost.big_step_tG ("_ \<Rightarrow>\<^sub>G\<^bsup> _ \<^esup> _" 55)
 end
 
 bundle no_big_stepG_syntax 
 begin
-no_notation BS_Generalized_Cost.big_step_tG ("_ \<Rightarrow>\<^bsup> _ \<^esup> _" 55)
+no_notation BS_Generalized_Cost.big_step_tG ("_ \<Rightarrow>\<^sub>G\<^bsup> _ \<^esup> _" 55)
 end
 
 (*
@@ -47,7 +50,7 @@ experiment
 begin
 
 text "finding out the final state and running time of a command:"
-schematic_goal ex: "(''x'' ::= A (N 5);; ''y'' ::= A (V ''x''), s) \<Rightarrow>\<^bsup> ?t \<^esup> ?s"
+schematic_goal ex: "(''x'' ::= A (N 5);; ''y'' ::= A (V ''x''), s) \<Rightarrow>\<^sub>G\<^bsup> ?t \<^esup> ?s"
   apply(rule Seq)
     apply(rule Assign)
    apply simp
@@ -58,76 +61,15 @@ schematic_goal ex: "(''x'' ::= A (N 5);; ''y'' ::= A (V ''x''), s) \<Rightarrow>
 
 values "{(t, x). big_step_t (SKIP, \<lambda>_. 0) x t}"
 
-values "{map t [''x''] |t x. (SKIP, <''x'' := 42>) \<Rightarrow>\<^bsup> x \<^esup> t}"
+values "{map t [''x''] |t x. (SKIP, <''x'' := 42>) \<Rightarrow>\<^sub>G\<^bsup> x \<^esup> t}"
 
-values "{map t [''x''] |t x. (''x'' ::=A (N 2), <''x'' := 42>) \<Rightarrow>\<^bsup> x \<^esup> t}"
+values "{map t [''x''] |t x. (''x'' ::=A (N 2), <''x'' := 42>) \<Rightarrow>\<^sub>G\<^bsup> x \<^esup> t}"
 
-values "{(map t [''x''],x) |t x. (WHILE ''x''\<noteq>0 DO ''x''::= Sub (V ''x'') (N 1),<''x'':=5>) \<Rightarrow>\<^bsup> x \<^esup> t }"
+values "{(map t [''x''],x) |t x. (WHILE ''x''\<noteq>0 DO ''x''::= Sub (V ''x'') (N 1),<''x'':=5>) \<Rightarrow>\<^sub>G\<^bsup> x \<^esup> t }"
 
 end
 
 *)
-
-subsection "Utilities"
-
-text "A more general, elegant version of those would be nice"
-
-lemma equality_lifted: "(\<lambda>x. y) = (\<lambda>x. z) \<longleftrightarrow> y = z"
-  by metis
-
-lemma add_left_cancel_lifted: "(\<lambda>x. (a :: 'a \<Rightarrow> nat) x + b x) = (\<lambda>x. a x + c x) \<longleftrightarrow> b = c"
-proof
-  assume "(\<lambda>x. a x + b x) = (\<lambda>x. a x + c x)" show "b = c"
-  proof(rule ccontr)
-    assume "b \<noteq> c"
-    have "(\<lambda>x. b x) \<noteq> (\<lambda>x. c x)"
-      by (simp add: \<open>b \<noteq> c\<close>)
-    hence "(\<lambda>x. a x + b x) \<noteq> (\<lambda>x. a x + c x)"
-      by (meson add_left_cancel)
-    thus False 
-      by (simp add: \<open>(\<lambda>x. a x + b x) = (\<lambda>x. a x + c x)\<close>)
-  qed
-next 
-  assume "b = c" show "(\<lambda>x. a x + b x) = (\<lambda>x. a x + c x)"
-    by (simp add: \<open>b = c\<close>)
-qed
-
-lemma add_right_cancel_lifted: "(\<lambda>x. (a :: 'a \<Rightarrow> nat) x + c x) = (\<lambda>x. b x + c x) \<longleftrightarrow> a = b"
-proof
-  assume "(\<lambda>x. a x + c x) = (\<lambda>x. b x + c x) " show "a = b"
-  proof(rule ccontr)
-    assume "a \<noteq> b"
-    have "(\<lambda>x. a x) \<noteq> (\<lambda>x. b x)"
-      by (simp add: \<open>a \<noteq> b\<close>)
-    hence "(\<lambda>x. a x + c x) \<noteq> (\<lambda>x. b x + c x)"
-      by (metis add.commute add_left_cancel)
-    thus False 
-      by (simp add: \<open>(\<lambda>x. a x + c x) = (\<lambda>x. b x + c x)\<close>)
-  qed
-next 
-  assume "a = b" show "(\<lambda>x. a x + c x) = (\<lambda>x. b x + c x)"
-    by (simp add: \<open>a = b\<close>)
-qed
-
-lemma Suc_inject_lifted: "(\<lambda>x. Suc (y x)) = (\<lambda>x. Suc (z x)) \<longleftrightarrow> y = z"
-proof
-  assume "(\<lambda>x. Suc (y x)) = (\<lambda>x. Suc (z x))" show "y = z"
-  proof(rule ccontr)
-    assume "y \<noteq> z"
-    have "(\<lambda>x. y x) \<noteq> (\<lambda>x. z x)"
-      by (simp add: \<open>y \<noteq> z\<close>)
-    hence "(\<lambda>x. Suc (y x)) \<noteq> (\<lambda>x. Suc (z x))"
-      by (meson nat.inject)
-    thus False 
-      by (simp add: \<open>(\<lambda>x. Suc (y x)) = (\<lambda>x. Suc (z x))\<close>)
-  qed
-next 
-  assume "y = z" show "(\<lambda>x. Suc (y x)) = (\<lambda>x. Suc (z x))"
-    by (simp add: \<open>y = z\<close>)
-qed
-
-lemma add_diff_cancel_right'_lifted [simp]: "(\<lambda>x. ((a :: 'a \<Rightarrow> nat) x + b x) - b x) = (\<lambda>x. a x)"
-  by simp
 
 context BS_Generalized_Cost begin
 
@@ -136,53 +78,58 @@ subsection "proof automation:"
 text "Introduction rules:"
 declare  BS_Generalized_Cost.big_step_tG.intros [intro]
 
+thm big_step_tG.induct
+
 text "Induction rules with pair splitting"
-lemmas big_step_tG_induct =  BS_Generalized_Cost.big_step_tG.induct[split_format(complete)]
+lemmas big_step_tG_induct = big_step_tG.induct[split_format(complete), OF BS_Generalized_Cost_axioms]
+
+lemma "(c, s) \<Rightarrow>\<^sub>G\<^bsup> C \<^esup> s' \<Longrightarrow> BS_Generalized_Cost.big_step_tG skip_costs assign_costs (c, s) C s'"
+  by simp
 
 subsection "Rule inversion"
-inductive_cases Skip_tE[elim!]: "(SKIP,s) \<Rightarrow>\<^bsup> C \<^esup> t"
-inductive_cases Assign_tE[elim!]: "(x ::= a,s) \<Rightarrow>\<^bsup> C \<^esup> t"
-inductive_cases Seq_tE[elim!]: "(c1;;c2,s1) \<Rightarrow>\<^bsup> C \<^esup> s2"
-inductive_cases If_tE[elim!]: "(IF b \<noteq>0 THEN c1 ELSE c2,s) \<Rightarrow>\<^bsup> C \<^esup> t"
-inductive_cases While_tE[elim]: "(WHILE b \<noteq>0 DO c,s) \<Rightarrow>\<^bsup> C \<^esup> t"
-lemma Seq': "\<lbrakk>(c1,s1) \<Rightarrow>\<^bsup> C1 \<^esup> s2;  (c2,s2) \<Rightarrow>\<^bsup> C2 \<^esup> s3\<rbrakk> \<Longrightarrow> (c1;;c2, s1) \<Rightarrow>\<^bsup> (\<lambda>x. C1 x + C2 x) \<^esup> s3"
+inductive_cases Skip_tE[elim!]: "(SKIP,s) \<Rightarrow>\<^sub>G\<^bsup> C \<^esup> t"
+inductive_cases Assign_tE[elim!]: "(x ::= a,s) \<Rightarrow>\<^sub>G\<^bsup> C \<^esup> t"
+inductive_cases Seq_tE[elim!]: "(c1;;c2,s1) \<Rightarrow>\<^sub>G\<^bsup> C \<^esup> s2"
+inductive_cases If_tE[elim!]: "(IF b \<noteq>0 THEN c1 ELSE c2,s) \<Rightarrow>\<^sub>G\<^bsup> C \<^esup> t"
+inductive_cases While_tE[elim]: "(WHILE b \<noteq>0 DO c,s) \<Rightarrow>\<^sub>G\<^bsup> C \<^esup> t"
+lemma Seq': "\<lbrakk>(c1,s1) \<Rightarrow>\<^sub>G\<^bsup> C1 \<^esup> s2;  (c2,s2) \<Rightarrow>\<^sub>G\<^bsup> C2 \<^esup> s3\<rbrakk> \<Longrightarrow> (c1;;c2, s1) \<Rightarrow>\<^sub>G\<^bsup> (\<lambda>x. C1 x + C2 x) \<^esup> s3"
   by (simp add: Seq)
-lemma While_tE': "\<lbrakk> s1 b \<noteq> 0;  (c,s1) \<Rightarrow>\<^bsup> C1 \<^esup> s2;  (WHILE b \<noteq>0 DO c, s2) \<Rightarrow>\<^bsup> C2 \<^esup> s3\<rbrakk> 
-    \<Longrightarrow> (WHILE b \<noteq>0 DO c, s1) \<Rightarrow>\<^bsup> (\<lambda>x. (C1 x) + (C2 x) + 1) \<^esup> s3"
+lemma While_tE': "\<lbrakk> s1 b \<noteq> 0;  (c,s1) \<Rightarrow>\<^sub>G\<^bsup> C1 \<^esup> s2;  (WHILE b \<noteq>0 DO c, s2) \<Rightarrow>\<^sub>G\<^bsup> C2 \<^esup> s3\<rbrakk> 
+    \<Longrightarrow> (WHILE b \<noteq>0 DO c, s1) \<Rightarrow>\<^sub>G\<^bsup> (\<lambda>x. (C1 x) + (C2 x) + 1) \<^esup> s3"
   by (simp add: big_step_tG.WhileTrue)
 
 thm Seq_tE
 
 
-lemma Seq_costs_split: "(c1;;c2, s1) \<Rightarrow>\<^bsup> C \<^esup> s3 \<Longrightarrow> \<exists>C1 C2 s2. ((c1,s1) \<Rightarrow>\<^bsup> C1 \<^esup> s2) \<and>  ((c2,s2) \<Rightarrow>\<^bsup> C2 \<^esup> s3) \<and> C = (\<lambda>x. (C1 x) + (C2 x))" 
+lemma Seq_costs_split: "(c1;;c2, s1) \<Rightarrow>\<^sub>G\<^bsup> C \<^esup> s3 \<Longrightarrow> \<exists>C1 C2 s2. ((c1,s1) \<Rightarrow>\<^sub>G\<^bsup> C1 \<^esup> s2) \<and>  ((c2,s2) \<Rightarrow>\<^sub>G\<^bsup> C2 \<^esup> s3) \<and> C = (\<lambda>x. (C1 x) + (C2 x))" 
   apply (erule Seq_tE)
   by auto
 
-lemma While_costs_split: "\<lbrakk> s1 b \<noteq> 0;  (WHILE b \<noteq>0 DO c, s1) \<Rightarrow>\<^bsup> C \<^esup> s3\<rbrakk> 
-    \<Longrightarrow> \<exists>C1 C2 s2. ((c,s1) \<Rightarrow>\<^bsup> C1 \<^esup> s2) \<and> ((WHILE b \<noteq>0 DO c, s2) \<Rightarrow>\<^bsup> C2 \<^esup> s3) \<and> C = (\<lambda>x. (C1 x) + (C2 x) + 1)"
+lemma While_costs_split: "\<lbrakk> s1 b \<noteq> 0;  (WHILE b \<noteq>0 DO c, s1) \<Rightarrow>\<^sub>G\<^bsup> C \<^esup> s3\<rbrakk> 
+    \<Longrightarrow> \<exists>C1 C2 s2. ((c,s1) \<Rightarrow>\<^sub>G\<^bsup> C1 \<^esup> s2) \<and> ((WHILE b \<noteq>0 DO c, s2) \<Rightarrow>\<^sub>G\<^bsup> C2 \<^esup> s3) \<and> C = (\<lambda>x. (C1 x) + (C2 x) + 1)"
   by force
 
 
 thm While_tE
 
 text "Rule inversion use examples:"
-lemma "(IF b \<noteq>0 THEN SKIP ELSE SKIP, s) \<Rightarrow>\<^bsup> C \<^esup> t \<Longrightarrow> t = s"
+lemma "(IF b \<noteq>0 THEN SKIP ELSE SKIP, s) \<Rightarrow>\<^sub>G\<^bsup> C \<^esup> t \<Longrightarrow> t = s"
   by blast
 
-lemma assumes "(IF b \<noteq>0 THEN SKIP ELSE SKIP, s) \<Rightarrow>\<^bsup> C \<^esup> t"
+lemma assumes "(IF b \<noteq>0 THEN SKIP ELSE SKIP, s) \<Rightarrow>\<^sub>G\<^bsup> C \<^esup> t"
   shows "t = s"
   using assms apply cases by auto
 
 lemma assign_t_simp:
-  "((x ::= a,s) \<Rightarrow>\<^bsup> assign_costs \<^esup>  s') \<longleftrightarrow> (s' = s(x := aval a s))"
+  "((x ::= a,s) \<Rightarrow>\<^sub>G\<^bsup> assign_costs \<^esup>  s') \<longleftrightarrow> (s' = s(x := aval a s))"
   using big_step_tG.Assign by auto
 
-lemma seq_costs_split: "(c1;;c2,s1) \<Rightarrow>\<^bsup> C \<^esup> s2 \<Longrightarrow> 
-                        \<exists>C1 C2 s. ((c1,s1) \<Rightarrow>\<^bsup> C1 \<^esup> s) \<and> ((c2,s) \<Rightarrow>\<^bsup> C2 \<^esup> s2)
+lemma seq_costs_split: "(c1;;c2,s1) \<Rightarrow>\<^sub>G\<^bsup> C \<^esup> s2 \<Longrightarrow> 
+                        \<exists>C1 C2 s. ((c1,s1) \<Rightarrow>\<^sub>G\<^bsup> C1 \<^esup> s) \<and> ((c2,s) \<Rightarrow>\<^sub>G\<^bsup> C2 \<^esup> s2)
                         \<and> C = (\<lambda>x. (C1 x) + (C2 x)) " by auto
 
 subsection "Determinism of Big semantics of IMP-"
-theorem big_step_t_state_determ2: "\<lbrakk> (c,s) \<Rightarrow>\<^bsup> p \<^esup> t; (c,s) \<Rightarrow>\<^bsup> q \<^esup> u \<rbrakk> \<Longrightarrow> (u = t)"
+theorem big_step_t_state_determ2: "\<lbrakk> (c,s) \<Rightarrow>\<^sub>G\<^bsup> p \<^esup> t; (c,s) \<Rightarrow>\<^sub>G\<^bsup> q \<^esup> u \<rbrakk> \<Longrightarrow> (u = t)"
   apply  (induction  arbitrary: u q rule: big_step_tG.induct)
     apply(elim Skip_tE) apply(simp)
     apply(elim Assign_tE) apply(simp)
@@ -206,7 +153,7 @@ theorem big_step_t_state_determ2: "\<lbrakk> (c,s) \<Rightarrow>\<^bsup> p \<^es
         using p(1-6) by (simp)
 done *)
 
-theorem big_step_t_cost_determ2: "\<lbrakk> (c,s) \<Rightarrow>\<^bsup> p \<^esup> t; (c,s) \<Rightarrow>\<^bsup> q \<^esup> t \<rbrakk> \<Longrightarrow> p = q"
+theorem big_step_t_cost_determ2: "\<lbrakk> (c,s) \<Rightarrow>\<^sub>G\<^bsup> p \<^esup> t; (c,s) \<Rightarrow>\<^sub>G\<^bsup> q \<^esup> t \<rbrakk> \<Longrightarrow> p = q"
 proof  (induction  arbitrary: q rule: big_step_tG.induct)
   case (Skip s)
   then show ?case 
@@ -240,27 +187,27 @@ next
   case (WhileTrue s1 b c C1 s2 C2 s3 C3)
   then show ?case  proof-
     obtain q1 q2 s2' where "
-   ((c, s1) \<Rightarrow>\<^bsup> q1 \<^esup> s2') \<and>
-   ((WHILE b\<noteq>0 DO c, s2') \<Rightarrow>\<^bsup> q2 \<^esup> s3) \<and> q = (\<lambda>x. q1 x + q2 x + 1)"
+   ((c, s1) \<Rightarrow>\<^sub>G\<^bsup> q1 \<^esup> s2') \<and>
+   ((WHILE b\<noteq>0 DO c, s2') \<Rightarrow>\<^sub>G\<^bsup> q2 \<^esup> s3) \<and> q = (\<lambda>x. q1 x + q2 x + 1)"
       using WhileTrue.hyps(1) WhileTrue.prems by auto
     have "s2' = s2" 
-      using WhileTrue.hyps(2) \<open>(c, s1) \<Rightarrow>\<^bsup> q1 \<^esup> s2' \<and> (WHILE b\<noteq>0 DO c, s2') \<Rightarrow>\<^bsup> q2 \<^esup> s3 \<and> q = (\<lambda>x. q1 x + q2 x + 1)\<close> big_step_t_state_determ2 by auto
+      using WhileTrue.hyps(2) \<open>((c, s1) \<Rightarrow>\<^sub>G\<^bsup> q1 \<^esup> s2') \<and> ((WHILE b\<noteq>0 DO c, s2') \<Rightarrow>\<^sub>G\<^bsup> q2 \<^esup> s3) \<and> q = (\<lambda>x. q1 x + q2 x + 1)\<close> big_step_t_state_determ2 by auto
     moreover have "q1 = C1"
-    proof- have "(c, s1) \<Rightarrow>\<^bsup> q1 \<^esup> s2" 
-        using \<open>(c, s1) \<Rightarrow>\<^bsup> q1 \<^esup> s2' \<and> (WHILE b\<noteq>0 DO c, s2') \<Rightarrow>\<^bsup> q2 \<^esup> s3 \<and> q = (\<lambda>x. q1 x + q2 x + 1)\<close> calculation by auto
+    proof- have "(c, s1) \<Rightarrow>\<^sub>G\<^bsup> q1 \<^esup> s2" 
+        using \<open>((c, s1) \<Rightarrow>\<^sub>G\<^bsup> q1 \<^esup> s2') \<and> ((WHILE b\<noteq>0 DO c, s2') \<Rightarrow>\<^sub>G\<^bsup> q2 \<^esup> s3) \<and> q = (\<lambda>x. q1 x + q2 x + 1)\<close> calculation by auto
       thus ?thesis 
         using WhileTrue.IH(1) by auto
     qed
     moreover have "q2 = C2"
-    proof- have "(WHILE b\<noteq>0 DO c, s2) \<Rightarrow>\<^bsup> q2 \<^esup> s3" 
-        using \<open>((c, s1) \<Rightarrow>\<^bsup> q1 \<^esup> s2') \<and>
-   ((WHILE b\<noteq>0 DO c, s2') \<Rightarrow>\<^bsup> q2 \<^esup> s3) \<and> q = (\<lambda>x. q1 x + q2 x + 1)\<close> calculation by auto
+    proof- have "(WHILE b\<noteq>0 DO c, s2) \<Rightarrow>\<^sub>G\<^bsup> q2 \<^esup> s3" 
+        using \<open>((c, s1) \<Rightarrow>\<^sub>G\<^bsup> q1 \<^esup> s2') \<and>
+   ((WHILE b\<noteq>0 DO c, s2') \<Rightarrow>\<^sub>G\<^bsup> q2 \<^esup> s3) \<and> q = (\<lambda>x. q1 x + q2 x + 1)\<close> calculation by auto
       thus ?thesis 
         by (simp add: WhileTrue.IH(2))
     qed
     moreover have "q = (\<lambda>x. C1 x + C2 x + 1)" 
     proof-
-      have " q = (\<lambda>x. q1 x + q2 x + 1)" using \<open>(c, s1) \<Rightarrow>\<^bsup> q1 \<^esup> s2' \<and> (WHILE b\<noteq>0 DO c, s2') \<Rightarrow>\<^bsup> q2 \<^esup> s3 \<and> q = (\<lambda>x. q1 x + q2 x + 1)\<close>
+      have " q = (\<lambda>x. q1 x + q2 x + 1)" using \<open>((c, s1) \<Rightarrow>\<^sub>G\<^bsup> q1 \<^esup> s2') \<and> ((WHILE b\<noteq>0 DO c, s2') \<Rightarrow>\<^sub>G\<^bsup> q2 \<^esup> s3) \<and> q = (\<lambda>x. q1 x + q2 x + 1)\<close>
         by simp
       thus ?thesis using calculation(2-3)
         by (simp add: \<open>q = (\<lambda>x. q1 x + q2 x + 1)\<close>)
@@ -270,43 +217,43 @@ next
   qed
 qed
 
-lemma bigstep_det: "(c1, s) \<Rightarrow>\<^bsup> p1 \<^esup> t1 \<Longrightarrow> (c1, s) \<Rightarrow>\<^bsup> p \<^esup> t \<Longrightarrow> p1 = p  \<and> t1=t"
+lemma bigstep_det: "(c1, s) \<Rightarrow>\<^sub>G\<^bsup> p1 \<^esup> t1 \<Longrightarrow> (c1, s) \<Rightarrow>\<^sub>G\<^bsup> p \<^esup> t \<Longrightarrow> p1 = p  \<and> t1=t"
   by (metis big_step_t_cost_determ2 big_step_t_state_determ2)
 
 
 lemma seq_assign_t_simp:
-  "((c ;; x ::= a, s) \<Rightarrow>\<^bsup> (\<lambda>x. t x + assign_costs x) \<^esup>  s') 
-  \<longleftrightarrow> (\<exists>s''. ((c, s) \<Rightarrow>\<^bsup> t \<^esup> s'') \<and> s' = s''(x := aval a s''))"
+  "((c ;; x ::= a, s) \<Rightarrow>\<^sub>G\<^bsup> (\<lambda>x. t x + assign_costs x) \<^esup>  s') 
+  \<longleftrightarrow> (\<exists>s''. ((c, s) \<Rightarrow>\<^sub>G\<^bsup> t \<^esup> s'') \<and> s' = s''(x := aval a s''))"
 proof
-  assume "(c;; x ::= a, s) \<Rightarrow>\<^bsup> (\<lambda>x. t x + assign_costs x) \<^esup> s'"
+  assume "(c;; x ::= a, s) \<Rightarrow>\<^sub>G\<^bsup> (\<lambda>x. t x + assign_costs x) \<^esup> s'"
   thm seq_costs_split
-  then obtain C1 C2 s'' where "(c, s) \<Rightarrow>\<^bsup> C1 \<^esup> s''" 
-                          and "(x ::= a, s'') \<Rightarrow>\<^bsup> C2 \<^esup> s'" 
+  then obtain C1 C2 s'' where "(c, s) \<Rightarrow>\<^sub>G\<^bsup> C1 \<^esup> s''" 
+                          and "(x ::= a, s'') \<Rightarrow>\<^sub>G\<^bsup> C2 \<^esup> s'" 
                           and " (\<lambda>x. t x + assign_costs x) = (\<lambda>x. C1 x + C2 x)"
-    using \<open>(c;; x ::= a, s) \<Rightarrow>\<^bsup> (\<lambda>x. t x + assign_costs x) \<^esup> s'\<close> seq_costs_split 
+    using \<open>(c;; x ::= a, s) \<Rightarrow>\<^sub>G\<^bsup> (\<lambda>x. t x + assign_costs x) \<^esup> s'\<close> seq_costs_split 
     by meson
-  have "assign_costs = C2" using \<open>(c;; x ::= a, s) \<Rightarrow>\<^bsup>  (\<lambda>x. t x + assign_costs x) \<^esup> s'\<close>
-    using \<open>(x ::= a, s'') \<Rightarrow>\<^bsup> C2 \<^esup> s'\<close> by auto
+  have "assign_costs = C2" using \<open>(c;; x ::= a, s) \<Rightarrow>\<^sub>G\<^bsup>  (\<lambda>x. t x + assign_costs x) \<^esup> s'\<close>
+    using \<open>(x ::= a, s'') \<Rightarrow>\<^sub>G\<^bsup> C2 \<^esup> s'\<close> by auto
   hence "(\<lambda>x. t x + assign_costs x) = (\<lambda>x. C1 x + assign_costs x)" 
     using \<open>(\<lambda>x. t x + assign_costs x) = (\<lambda>x. C1 x + C2 x)\<close> by auto 
   hence "t = C1" using add_right_cancel_lifted by auto
-  thus "\<exists>s''. ((c, s) \<Rightarrow>\<^bsup> t \<^esup> s'') \<and> s' = s''(x := aval a s'')"
-    using \<open>(c, s) \<Rightarrow>\<^bsup> C1 \<^esup> s''\<close> \<open>(x ::= a, s'') \<Rightarrow>\<^bsup> C2 \<^esup> s'\<close> by auto
+  thus "\<exists>s''. ((c, s) \<Rightarrow>\<^sub>G\<^bsup> t \<^esup> s'') \<and> s' = s''(x := aval a s'')"
+    using \<open>(c, s) \<Rightarrow>\<^sub>G\<^bsup> C1 \<^esup> s''\<close> \<open>(x ::= a, s'') \<Rightarrow>\<^sub>G\<^bsup> C2 \<^esup> s'\<close> by auto
 next
-  assume "\<exists>s''. ((c, s) \<Rightarrow>\<^bsup> t \<^esup> s'') \<and> s' = s''(x := aval a s'')"
-  thus "(c ;; x ::= a, s) \<Rightarrow>\<^bsup> (\<lambda>x. t x + assign_costs x) \<^esup>  s'"
+  assume "\<exists>s''. ((c, s) \<Rightarrow>\<^sub>G\<^bsup> t \<^esup> s'') \<and> s' = s''(x := aval a s'')"
+  thus "(c ;; x ::= a, s) \<Rightarrow>\<^sub>G\<^bsup> (\<lambda>x. t x + assign_costs x) \<^esup>  s'"
     using Seq' big_step_tG.Assign by auto
 qed 
 
-lemma seq_assign_t_intro: "(c, s) \<Rightarrow>\<^bsup> t \<^esup> s'' \<Longrightarrow> s' = s''(x := aval a s'')
-  \<Longrightarrow>(c ;; x ::= a, s) \<Rightarrow>\<^bsup> (\<lambda>x. t x + assign_costs x) \<^esup>  s'"
+lemma seq_assign_t_intro: "(c, s) \<Rightarrow>\<^sub>G\<^bsup> t \<^esup> s'' \<Longrightarrow> s' = s''(x := aval a s'')
+  \<Longrightarrow>(c ;; x ::= a, s) \<Rightarrow>\<^sub>G\<^bsup> (\<lambda>x. t x + assign_costs x) \<^esup>  s'"
   using seq_assign_t_simp 
   by auto
 
-lemma seq_is_noop[simp]: "((SKIP, s) \<Rightarrow>\<^bsup>t\<^esup> s') \<longleftrightarrow> (t = skip_costs \<and> s = s')" 
+lemma seq_is_noop[simp]: "((SKIP, s) \<Rightarrow>\<^sub>G\<^bsup>t\<^esup> s') \<longleftrightarrow> (t = skip_costs \<and> s = s')" 
   using Skip by auto
 
-lemma seq_skip[simp]: "((c ;; SKIP, s) \<Rightarrow>\<^bsup>(\<lambda>x. t x + skip_costs x)\<^esup> s') \<longleftrightarrow> ((c, s) \<Rightarrow>\<^bsup>t\<^esup> s')"
+lemma seq_skip[simp]: "((c ;; SKIP, s) \<Rightarrow>\<^sub>G\<^bsup>(\<lambda>x. t x + skip_costs x)\<^esup> s') \<longleftrightarrow> ((c, s) \<Rightarrow>\<^sub>G\<^bsup>t\<^esup> s')"
   apply auto 
   apply (simp add: add_right_cancel_lifted)
   by (simp add: Seq')
@@ -316,22 +263,22 @@ text "every command costs time"
 
 (* Needs extra skip assumption to hold, not sure if we want it for the general case *)
 
-lemma bigstep_progress:  "(c, s) \<Rightarrow>\<^bsup> p \<^esup> t \<Longrightarrow> \<forall>x. skip_costs x > 0 \<Longrightarrow>  \<forall>x. p x > 0"
+lemma bigstep_progress:  "(c, s) \<Rightarrow>\<^sub>G\<^bsup> p \<^esup> t \<Longrightarrow> \<forall>x. skip_costs x > 0 \<Longrightarrow>  \<forall>x. p x > 0"
   apply(induct rule: big_step_tG.induct, auto)
   by (simp add: assign_cost_positive)
 
 subsection "abbreviations and properties"
-abbreviation terminates ("\<down>") where "terminates cs \<equiv> (\<exists>n a. (cs \<Rightarrow>\<^bsup> n \<^esup> a))"
-abbreviation thestate ("\<down>\<^sub>s") where "thestate cs \<equiv> (THE a. \<exists>n. (cs \<Rightarrow>\<^bsup> n \<^esup> a))" 
-abbreviation thetime ("\<down>\<^sub>t") where "thetime cs \<equiv> (THE n. \<exists>a. (cs \<Rightarrow>\<^bsup> n \<^esup> a))"
+abbreviation terminates ("\<down>") where "terminates cs \<equiv> (\<exists>n a. (cs \<Rightarrow>\<^sub>G\<^bsup> n \<^esup> a))"
+abbreviation thestate ("\<down>\<^sub>s") where "thestate cs \<equiv> (THE a. \<exists>n. (cs \<Rightarrow>\<^sub>G\<^bsup> n \<^esup> a))" 
+abbreviation thetime ("\<down>\<^sub>t") where "thetime cs \<equiv> (THE n. \<exists>a. (cs \<Rightarrow>\<^sub>G\<^bsup> n \<^esup> a))"
 
-lemma bigstepT_the_cost: "(c, s) \<Rightarrow>\<^bsup> t \<^esup> s' \<Longrightarrow> \<down>\<^sub>t(c, s) = t"
+lemma bigstepT_the_cost: "(c, s) \<Rightarrow>\<^sub>G\<^bsup> t \<^esup> s' \<Longrightarrow> \<down>\<^sub>t(c, s) = t"
   using bigstep_det by blast 
 
-lemma bigstepT_the_state: "(c, s) \<Rightarrow>\<^bsup> t \<^esup> s' \<Longrightarrow> \<down>\<^sub>s(c, s) = s'"
+lemma bigstepT_the_state: "(c, s) \<Rightarrow>\<^sub>G\<^bsup> t \<^esup> s' \<Longrightarrow> \<down>\<^sub>s(c, s) = s'"
   using bigstep_det by blast 
 
-lemma SKIPnot: "(\<not> ((SKIP, s) \<Rightarrow>\<^bsup> p \<^esup> t)) \<longleftrightarrow> (s\<noteq>t \<or> p\<noteq>skip_costs)" by auto
+lemma SKIPnot: "(\<not> ((SKIP, s) \<Rightarrow>\<^sub>G\<^bsup> p \<^esup> t)) \<longleftrightarrow> (s\<noteq>t \<or> p\<noteq>skip_costs)" by auto
 
 lemma SKIPp: "\<down>\<^sub>t(SKIP,s) = skip_costs"
   apply(rule the_equality)
@@ -346,116 +293,116 @@ lemma ASSp: "(THE p. Ex (big_step_tG (x ::= e, s) p)) = assign_costs"
   apply auto 
   using big_step_tG.Assign by auto  
 
-lemma ASSt: "(THE t. \<exists>p. ((x ::= e, s) \<Rightarrow>\<^bsup> p \<^esup> t)) = s(x := aval e s)"
+lemma ASSt: "(THE t. \<exists>p. ((x ::= e, s) \<Rightarrow>\<^sub>G\<^bsup> p \<^esup> t)) = s(x := aval e s)"
   apply(rule the_equality)
   apply auto 
   using big_step_tG.Assign by auto
 
-lemma ASSnot: "( \<not>((x ::= e, s) \<Rightarrow>\<^bsup> p \<^esup> t )) = (p\<noteq>assign_costs \<or> t\<noteq>s(x := aval e s))"
+lemma ASSnot: "( \<not>((x ::= e, s) \<Rightarrow>\<^sub>G\<^bsup> p \<^esup> t )) = (p\<noteq>assign_costs \<or> t\<noteq>s(x := aval e s))"
   apply auto
   by (simp add: big_step_tG.Assign)
 
 (*
-lemma If_THE_True: "Suc (THE n. \<exists>a. (c1, s) \<Rightarrow>\<^bsup> n \<^esup> a) =  (THE n. \<exists>a. (IF b \<noteq>0 THEN c1 ELSE c2, s) \<Rightarrow>\<^bsup> n \<^esup> a)"
+lemma If_THE_True: "Suc (THE n. \<exists>a. (c1, s) \<Rightarrow>\<^sub>G\<^bsup> n \<^esup> a) =  (THE n. \<exists>a. (IF b \<noteq>0 THEN c1 ELSE c2, s) \<Rightarrow>\<^sub>G\<^bsup> n \<^esup> a)"
      if T: "s b \<noteq> 0" and c1_t: "terminates (c1,s)" for s l
 proof -
-  from c1_t obtain p t where a: "(c1, s) \<Rightarrow>\<^bsup> p \<^esup> t" by blast
-  with T have b: "(IF b \<noteq>0 THEN c1 ELSE c2, s) \<Rightarrow>\<^bsup> p+1 \<^esup> t"  using IfTrue by simp
-  from a bigstepT_the_cost have "(THE n. \<exists>a. (c1, s) \<Rightarrow>\<^bsup> n \<^esup> a) = p" by simp
-  moreover from b bigstepT_the_cost have "(THE n. \<exists>a. (IF b \<noteq>0 THEN c1 ELSE c2, s) \<Rightarrow>\<^bsup> n \<^esup> a) = p+1" by simp
+  from c1_t obtain p t where a: "(c1, s) \<Rightarrow>\<^sub>G\<^bsup> p \<^esup> t" by blast
+  with T have b: "(IF b \<noteq>0 THEN c1 ELSE c2, s) \<Rightarrow>\<^sub>G\<^bsup> p+1 \<^esup> t"  using IfTrue by simp
+  from a bigstepT_the_cost have "(THE n. \<exists>a. (c1, s) \<Rightarrow>\<^sub>G\<^bsup> n \<^esup> a) = p" by simp
+  moreover from b bigstepT_the_cost have "(THE n. \<exists>a. (IF b \<noteq>0 THEN c1 ELSE c2, s) \<Rightarrow>\<^sub>G\<^bsup> n \<^esup> a) = p+1" by simp
   ultimately show ?thesis by simp
 qed
 
 lemma If_THE_False:
- "Suc (THE n. \<exists>a. (c2, s) \<Rightarrow>\<^bsup> n \<^esup> a) =  (THE n. \<exists>a. (IF b \<noteq>0 THEN c1 ELSE c2, s) \<Rightarrow>\<^bsup> n \<^esup> a)"
+ "Suc (THE n. \<exists>a. (c2, s) \<Rightarrow>\<^sub>G\<^bsup> n \<^esup> a) =  (THE n. \<exists>a. (IF b \<noteq>0 THEN c1 ELSE c2, s) \<Rightarrow>\<^sub>G\<^bsup> n \<^esup> a)"
      if T: "s b = 0" and c2_t: "\<down> (c2,s)" for s l
 proof -
-  from c2_t obtain p t where a: "(c2, s) \<Rightarrow>\<^bsup> p \<^esup> t"  by blast
-  with T have b: "(IF b \<noteq>0 THEN c1 ELSE c2, s) \<Rightarrow>\<^bsup> p+1 \<^esup> t"  using IfFalse by simp
-  from a bigstepT_the_cost have "(THE n. \<exists>a. (c2, s) \<Rightarrow>\<^bsup> n \<^esup> a) = p" by simp
-  moreover from b bigstepT_the_cost have "(THE n. \<exists>a. (IF b \<noteq>0 THEN c1 ELSE c2, s) \<Rightarrow>\<^bsup> n \<^esup> a) = p+1" by simp
+  from c2_t obtain p t where a: "(c2, s) \<Rightarrow>\<^sub>G\<^bsup> p \<^esup> t"  by blast
+  with T have b: "(IF b \<noteq>0 THEN c1 ELSE c2, s) \<Rightarrow>\<^sub>G\<^bsup> p+1 \<^esup> t"  using IfFalse by simp
+  from a bigstepT_the_cost have "(THE n. \<exists>a. (c2, s) \<Rightarrow>\<^sub>G\<^bsup> n \<^esup> a) = p" by simp
+  moreover from b bigstepT_the_cost have "(THE n. \<exists>a. (IF b \<noteq>0 THEN c1 ELSE c2, s) \<Rightarrow>\<^sub>G\<^bsup> n \<^esup> a) = p+1" by simp
   ultimately show ?thesis by simp
 qed
 
 *)
 
-lemma terminates_in_state_intro: "(c, s) \<Rightarrow>\<^bsup>t\<^esup> s' \<Longrightarrow> s' = s'' \<Longrightarrow> (c, s) \<Rightarrow>\<^bsup>t\<^esup> s''"
+lemma terminates_in_state_intro: "(c, s) \<Rightarrow>\<^sub>G\<^bsup>t\<^esup> s' \<Longrightarrow> s' = s'' \<Longrightarrow> (c, s) \<Rightarrow>\<^sub>G\<^bsup>t\<^esup> s''"
   by simp
 
-lemma terminates_in_time_state_intro: "(c, s) \<Rightarrow>\<^bsup>t\<^esup> s' \<Longrightarrow> t = t' \<Longrightarrow> s' = s'' 
-  \<Longrightarrow> (c, s) \<Rightarrow>\<^bsup>t'\<^esup> s''"
+lemma terminates_in_time_state_intro: "(c, s) \<Rightarrow>\<^sub>G\<^bsup>t\<^esup> s' \<Longrightarrow> t = t' \<Longrightarrow> s' = s'' 
+  \<Longrightarrow> (c, s) \<Rightarrow>\<^sub>G\<^bsup>t'\<^esup> s''"
   by simp
 
-lemma terminates_in_time_state_intro': "(c', s) \<Rightarrow>\<^bsup>t\<^esup> s' \<Longrightarrow> t = t' \<Longrightarrow> s' = s'' \<Longrightarrow> c' = c
-  \<Longrightarrow> (c, s) \<Rightarrow>\<^bsup>t'\<^esup> s''"
+lemma terminates_in_time_state_intro': "(c', s) \<Rightarrow>\<^sub>G\<^bsup>t\<^esup> s' \<Longrightarrow> t = t' \<Longrightarrow> s' = s'' \<Longrightarrow> c' = c
+  \<Longrightarrow> (c, s) \<Rightarrow>\<^sub>G\<^bsup>t'\<^esup> s''"
   by simp
 
 method dest_com  = 
-  (match premises in a: "\<lbrakk>loop_cond; state_upd\<rbrakk> \<Longrightarrow> (_, s) \<Rightarrow>\<^bsup>t\<^esup> s'"
+  (match premises in a: "\<lbrakk>loop_cond; state_upd\<rbrakk> \<Longrightarrow> (_, s) \<Rightarrow>\<^sub>G\<^bsup>t\<^esup> s'"
     for s s' t loop_cond state_upd \<Rightarrow> \<open>rule terminates_in_time_state_intro'[OF a]\<close>)
 
 method dest_com' = 
-  (match premises in a[thin]: "\<lbrakk>loop_cond; state_upd; (_, s) \<Rightarrow>\<^bsup>t\<^esup> s'\<rbrakk> \<Longrightarrow> P" 
+  (match premises in a[thin]: "\<lbrakk>loop_cond; state_upd; (_, s) \<Rightarrow>\<^sub>G\<^bsup>t\<^esup> s'\<rbrakk> \<Longrightarrow> P" 
     for s s' t loop_cond state_upd P  \<Rightarrow>
-   \<open>match premises in b[thin]: "(While _ _, s2) \<Rightarrow>\<^bsup>t2\<^esup> s2'"
+   \<open>match premises in b[thin]: "(While _ _, s2) \<Rightarrow>\<^sub>G\<^bsup>t2\<^esup> s2'"
       for s2 s2' t2 \<Rightarrow> \<open>insert a[OF _ _ b]\<close>\<close>)
 
 
 method dest_com_init_while = 
-  (match premises in a[thin]: "\<lbrakk>loop_cond; state_upd; ((_ ;; While _ _), s) \<Rightarrow>\<^bsup>t\<^esup> s'\<rbrakk> \<Longrightarrow> P" 
+  (match premises in a[thin]: "\<lbrakk>loop_cond; state_upd; ((_ ;; While _ _), s) \<Rightarrow>\<^sub>G\<^bsup>t\<^esup> s'\<rbrakk> \<Longrightarrow> P" 
     for s s' t loop_cond state_upd P  \<Rightarrow>
-   \<open>match premises in b[thin]: "((_ ;; While _ _), s2) \<Rightarrow>\<^bsup>t2\<^esup> s2'"
+   \<open>match premises in b[thin]: "((_ ;; While _ _), s2) \<Rightarrow>\<^sub>G\<^bsup>t2\<^esup> s2'"
       for s2 s2' t2 \<Rightarrow> \<open>insert a[OF _ _ b]\<close>\<close>)
 
 (*method dest_com_init_while = 
-  (match premises in a[thin]: "\<lbrakk>loop_cond; state_upd; (v ::= a;; WHILE v \<noteq>0 DO _, s) \<Rightarrow>\<^bsup>t\<^esup> s'\<rbrakk> \<Longrightarrow> P" 
+  (match premises in a[thin]: "\<lbrakk>loop_cond; state_upd; (v ::= a;; WHILE v \<noteq>0 DO _, s) \<Rightarrow>\<^sub>G\<^bsup>t\<^esup> s'\<rbrakk> \<Longrightarrow> P" 
     for v a s s' t loop_cond state_upd P  \<Rightarrow>
-   \<open>match premises in b[thin]: "(v ::= a;; WHILE v \<noteq>0 DO _, s2) \<Rightarrow>\<^bsup>t2\<^esup> s2'"
+   \<open>match premises in b[thin]: "(v ::= a;; WHILE v \<noteq>0 DO _, s2) \<Rightarrow>\<^sub>G\<^bsup>t2\<^esup> s2'"
       for s2 s2' t2 \<Rightarrow> \<open>insert a\<close>\<close>)*)
 
-lemma terminates_split_if : "(P s \<Longrightarrow> (c, s) \<Rightarrow>\<^bsup>t1\<^esup> s1 ) \<Longrightarrow> 
-(\<not> P s \<Longrightarrow> (c, s) \<Rightarrow>\<^bsup>t2\<^esup> s2 ) \<Longrightarrow> (c,s) \<Rightarrow>\<^bsup>if P s then t1 else t2\<^esup>  if P s then s1 else s2"
+lemma terminates_split_if : "(P s \<Longrightarrow> (c, s) \<Rightarrow>\<^sub>G\<^bsup>t1\<^esup> s1 ) \<Longrightarrow> 
+(\<not> P s \<Longrightarrow> (c, s) \<Rightarrow>\<^sub>G\<^bsup>t2\<^esup> s2 ) \<Longrightarrow> (c,s) \<Rightarrow>\<^sub>G\<^bsup>if P s then t1 else t2\<^esup>  if P s then s1 else s2"
   by auto
 
 lemma AssignD': 
-"(x ::= a, s) \<Rightarrow>\<^bsup> assign_costs \<^esup> s' \<Longrightarrow> s' = s (x:= aval a s)"
+"(x ::= a, s) \<Rightarrow>\<^sub>G\<^bsup> assign_costs \<^esup> s' \<Longrightarrow> s' = s (x:= aval a s)"
   by (auto simp add: eval_nat_numeral)
 
 (* TODO: Probably needs induction with pairs, needs fixing *)
-lemma com_only_vars: "\<lbrakk>(c, s) \<Rightarrow>\<^bsup> t \<^esup> s'; x \<notin> set (Max_Constant.all_variables c)\<rbrakk> \<Longrightarrow> s x = s' x"
+lemma com_only_vars: "\<lbrakk>(c, s) \<Rightarrow>\<^sub>G\<^bsup> t \<^esup> s'; x \<notin> set (Max_Constant.all_variables c)\<rbrakk> \<Longrightarrow> s x = s' x"
   apply (induction arbitrary: x rule: big_step_tG.induct) 
   oops
 
-lemma Seq'': "\<lbrakk> ((c1,s1) \<Rightarrow>\<^bsup> x \<^esup> s2) \<and> P s2; P s2 \<Longrightarrow> ((c2,s2) \<Rightarrow>\<^bsup> y \<^esup> s3) \<and> Q s3; Q s3 \<Longrightarrow> R s3 \<rbrakk>
-             \<Longrightarrow> ((c1;;c2, s1) \<Rightarrow>\<^bsup> (\<lambda>z. (x z) + (y z))\<^esup> s3) \<and> R s3"
+lemma Seq'': "\<lbrakk> ((c1,s1) \<Rightarrow>\<^sub>G\<^bsup> x \<^esup> s2) \<and> P s2; P s2 \<Longrightarrow> ((c2,s2) \<Rightarrow>\<^sub>G\<^bsup> y \<^esup> s3) \<and> Q s3; Q s3 \<Longrightarrow> R s3 \<rbrakk>
+             \<Longrightarrow> ((c1;;c2, s1) \<Rightarrow>\<^sub>G\<^bsup> (\<lambda>z. (x z) + (y z))\<^esup> s3) \<and> R s3"
   apply auto by (simp add: Seq')
 
 lemma WhileI:
-"\<lbrakk>(s1 b \<noteq> 0 \<Longrightarrow> ((c,s1) \<Rightarrow>\<^bsup> x \<^esup> s2) \<and> ((WHILE b \<noteq>0 DO c, s2) \<Rightarrow>\<^bsup> y \<^esup> s3));
+"\<lbrakk>(s1 b \<noteq> 0 \<Longrightarrow> ((c,s1) \<Rightarrow>\<^sub>G\<^bsup> x \<^esup> s2) \<and> ((WHILE b \<noteq>0 DO c, s2) \<Rightarrow>\<^sub>G\<^bsup> y \<^esup> s3));
   (s1 b = 0 \<Longrightarrow> s1 = s3);
   z = (if s1 b \<noteq> 0 then (\<lambda>z. (x z) + (y z) + 1) else (\<lambda>x. 2 * (skip_costs x)))\<rbrakk>
-        \<Longrightarrow> (WHILE b \<noteq>0 DO c, s1) \<Rightarrow>\<^bsup> z \<^esup> s3" 
+        \<Longrightarrow> (WHILE b \<noteq>0 DO c, s1) \<Rightarrow>\<^sub>G\<^bsup> z \<^esup> s3" 
   using WhileTrue 
    apply auto[1]
   using WhileFalse
   by simp
 
 lemma IfI:
-"\<lbrakk>s b \<noteq> 0 \<Longrightarrow> (c1,s) \<Rightarrow>\<^bsup> x1 \<^esup> t1;
-  s b = 0 \<Longrightarrow> (c2,s) \<Rightarrow>\<^bsup> x2 \<^esup> t2;
+"\<lbrakk>s b \<noteq> 0 \<Longrightarrow> (c1,s) \<Rightarrow>\<^sub>G\<^bsup> x1 \<^esup> t1;
+  s b = 0 \<Longrightarrow> (c2,s) \<Rightarrow>\<^sub>G\<^bsup> x2 \<^esup> t2;
   y = (\<lambda>x. (if s b \<noteq> 0 then x1 else x2) x + 1);
   t = (if s b \<noteq> 0 then t1 else t2)\<rbrakk>
-        \<Longrightarrow> (IF b \<noteq>0 THEN c1 ELSE c2, s) \<Rightarrow>\<^bsup> y \<^esup> t" 
+        \<Longrightarrow> (IF b \<noteq>0 THEN c1 ELSE c2, s) \<Rightarrow>\<^sub>G\<^bsup> y \<^esup> t" 
   by (auto simp add: IfTrue IfFalse)
 
 thm Suc_inject
 
 lemma IfE: 
-"(IF b \<noteq>0 THEN c1 ELSE c2, s) \<Rightarrow>\<^bsup> (\<lambda>x. (if s b \<noteq> 0 then x1 else x2) x + 1) \<^esup> (if s b \<noteq> 0 then s1 else s2) \<Longrightarrow> 
+"(IF b \<noteq>0 THEN c1 ELSE c2, s) \<Rightarrow>\<^sub>G\<^bsup> (\<lambda>x. (if s b \<noteq> 0 then x1 else x2) x + 1) \<^esup> (if s b \<noteq> 0 then s1 else s2) \<Longrightarrow> 
  \<lbrakk>\<lbrakk>s b \<noteq> 0; (\<lambda>x. (if s b \<noteq> 0 then x1 else x2) x + 1) = (\<lambda>x. x1 x + 1); 
-  (if s b \<noteq> 0 then s1 else s2) = s1; (c1,s) \<Rightarrow>\<^bsup> x1 \<^esup> s1\<rbrakk> \<Longrightarrow> P;
+  (if s b \<noteq> 0 then s1 else s2) = s1; (c1,s) \<Rightarrow>\<^sub>G\<^bsup> x1 \<^esup> s1\<rbrakk> \<Longrightarrow> P;
   \<lbrakk>s b = 0; (\<lambda>x. (if s b \<noteq> 0 then x1 else x2) x + 1) = (\<lambda>x. x2 x + 1);
-   (if s b \<noteq> 0 then s1 else s2) = s2; (c2,s) \<Rightarrow>\<^bsup> x2 \<^esup> s2\<rbrakk> \<Longrightarrow> P\<rbrakk>
+   (if s b \<noteq> 0 then s1 else s2) = s2; (c2,s) \<Rightarrow>\<^sub>G\<^bsup> x2 \<^esup> s2\<rbrakk> \<Longrightarrow> P\<rbrakk>
         \<Longrightarrow> P"
   apply (auto simp add: IfTrue IfFalse) 
    apply (metis add_right_cancel_lifted old.nat.inject)
@@ -463,9 +410,9 @@ lemma IfE:
 thm Seq_tE
 
 lemma IfD:
-"(IF b \<noteq>0 THEN c1 ELSE c2, s) \<Rightarrow>\<^bsup> (\<lambda>x. (if s b \<noteq> 0 then x1 else x2) x + 1) \<^esup> (if s b \<noteq> 0 then t1 else t2) \<Longrightarrow> 
- \<lbrakk>\<lbrakk>s b \<noteq> 0; (c1,s) \<Rightarrow>\<^bsup> x1 \<^esup> t1\<rbrakk> \<Longrightarrow> P;
-  \<lbrakk>s b = 0; (c2,s) \<Rightarrow>\<^bsup> x2 \<^esup> t2\<rbrakk> \<Longrightarrow> P\<rbrakk>
+"(IF b \<noteq>0 THEN c1 ELSE c2, s) \<Rightarrow>\<^sub>G\<^bsup> (\<lambda>x. (if s b \<noteq> 0 then x1 else x2) x + 1) \<^esup> (if s b \<noteq> 0 then t1 else t2) \<Longrightarrow> 
+ \<lbrakk>\<lbrakk>s b \<noteq> 0; (c1,s) \<Rightarrow>\<^sub>G\<^bsup> x1 \<^esup> t1\<rbrakk> \<Longrightarrow> P;
+  \<lbrakk>s b = 0; (c2,s) \<Rightarrow>\<^sub>G\<^bsup> x2 \<^esup> t2\<rbrakk> \<Longrightarrow> P\<rbrakk>
         \<Longrightarrow> P" 
   apply (auto simp add: IfTrue IfFalse)
    apply (metis add_right_cancel_lifted old.nat.inject) 
@@ -473,43 +420,43 @@ lemma IfD:
 
 lemma AssignI:
 "\<lbrakk>s' = s (x:= aval a s)\<rbrakk>
-        \<Longrightarrow> (x ::= a, s) \<Rightarrow>\<^bsup> assign_costs \<^esup> s'" 
+        \<Longrightarrow> (x ::= a, s) \<Rightarrow>\<^sub>G\<^bsup> assign_costs \<^esup> s'" 
   by (auto simp add: Assign)
 
 lemma AssignI': 
 "\<lbrakk>s' = s (x:= aval a s)\<rbrakk>
-        \<Longrightarrow> (x ::= a, s) \<Rightarrow>\<^bsup> assign_costs \<^esup> s'" 
+        \<Longrightarrow> (x ::= a, s) \<Rightarrow>\<^sub>G\<^bsup> assign_costs \<^esup> s'" 
   by (auto simp add: Assign eval_nat_numeral)
 
 lemma AssignI'': 
 "\<lbrakk>s' = s (x:= aval a s)\<rbrakk>
-        \<Longrightarrow> ((x ::= a, s) \<Rightarrow>\<^bsup> assign_costs \<^esup> s') \<and> (s' = s')" 
+        \<Longrightarrow> ((x ::= a, s) \<Rightarrow>\<^sub>G\<^bsup> assign_costs \<^esup> s') \<and> (s' = s')" 
   by (auto simp add: Assign eval_nat_numeral)
 
-lemma AssignD: "(x ::= a, s) \<Rightarrow>\<^bsup> t \<^esup> s' \<Longrightarrow> t = assign_costs \<and> s' = s(x := aval a s)"
+lemma AssignD: "(x ::= a, s) \<Rightarrow>\<^sub>G\<^bsup> t \<^esup> s' \<Longrightarrow> t = assign_costs \<and> s' = s(x := aval a s)"
   by auto
 
 lemma compose_programs_1:
-  "(c2, s2) \<Rightarrow>\<^bsup> y \<^esup> s3 \<Longrightarrow> (c1, s1) \<Rightarrow>\<^bsup> x \<^esup> s2 \<Longrightarrow> 
-    ((c1;; c2, s1) \<Rightarrow>\<^bsup> (\<lambda>z. x z + y z) \<^esup> s3 \<Longrightarrow> P)
+  "(c2, s2) \<Rightarrow>\<^sub>G\<^bsup> y \<^esup> s3 \<Longrightarrow> (c1, s1) \<Rightarrow>\<^sub>G\<^bsup> x \<^esup> s2 \<Longrightarrow> 
+    ((c1;; c2, s1) \<Rightarrow>\<^sub>G\<^bsup> (\<lambda>z. x z + y z) \<^esup> s3 \<Longrightarrow> P)
    \<Longrightarrow> P" 
   by (simp add: Seq')
 
 lemma compose_programs_2:
-  "(c1, s1) \<Rightarrow>\<^bsup> x \<^esup> s2 \<Longrightarrow> (c2, s2) \<Rightarrow>\<^bsup> y \<^esup> s3 \<Longrightarrow> 
-    ((c1;; c2, s1) \<Rightarrow>\<^bsup> (\<lambda>z. x z + y z) \<^esup> s3 \<Longrightarrow> P)
+  "(c1, s1) \<Rightarrow>\<^sub>G\<^bsup> x \<^esup> s2 \<Longrightarrow> (c2, s2) \<Rightarrow>\<^sub>G\<^bsup> y \<^esup> s3 \<Longrightarrow> 
+    ((c1;; c2, s1) \<Rightarrow>\<^sub>G\<^bsup> (\<lambda>z. x z + y z) \<^esup> s3 \<Longrightarrow> P)
    \<Longrightarrow> P"
   by (simp add: Seq')
 
 lemma While_tE_time:
-"(WHILE b\<noteq>0 DO c, s) \<Rightarrow>\<^bsup> x \<^esup> t \<Longrightarrow>
+"(WHILE b\<noteq>0 DO c, s) \<Rightarrow>\<^sub>G\<^bsup> x \<^esup> t \<Longrightarrow>
   (x = (\<lambda>x. 2 * (skip_costs x)) \<Longrightarrow> t = s \<Longrightarrow> s b = 0 \<Longrightarrow> P) \<Longrightarrow>
-  (\<And>x' s2 y. 0 < s b \<Longrightarrow> (c, s) \<Rightarrow>\<^bsup> x' \<^esup> s2 \<Longrightarrow> (WHILE b\<noteq>0 DO c, s2) \<Rightarrow>\<^bsup> y \<^esup> t \<Longrightarrow> x = (\<lambda>z. x' z + y z + 1) \<Longrightarrow> P) \<Longrightarrow> P"
+  (\<And>x' s2 y. 0 < s b \<Longrightarrow> (c, s) \<Rightarrow>\<^sub>G\<^bsup> x' \<^esup> s2 \<Longrightarrow> (WHILE b\<noteq>0 DO c, s2) \<Rightarrow>\<^sub>G\<^bsup> y \<^esup> t \<Longrightarrow> x = (\<lambda>z. x' z + y z + 1) \<Longrightarrow> P) \<Longrightarrow> P"
   by auto
 
 lemma Seq_tE_While_init:
-  "(WHILE v \<noteq>0 DO c2, s2) \<Rightarrow>\<^bsup> y \<^esup> s3 \<Longrightarrow> (c1, s1) \<Rightarrow>\<^bsup> x \<^esup> s2 \<Longrightarrow> 
-    ((c1;; WHILE v \<noteq>0 DO c2, s1) \<Rightarrow>\<^bsup> (\<lambda>z. x z + y z) \<^esup> s3 \<Longrightarrow> P)
+  "(WHILE v \<noteq>0 DO c2, s2) \<Rightarrow>\<^sub>G\<^bsup> y \<^esup> s3 \<Longrightarrow> (c1, s1) \<Rightarrow>\<^sub>G\<^bsup> x \<^esup> s2 \<Longrightarrow> 
+    ((c1;; WHILE v \<noteq>0 DO c2, s1) \<Rightarrow>\<^sub>G\<^bsup> (\<lambda>z. x z + y z) \<^esup> s3 \<Longrightarrow> P)
    \<Longrightarrow> P"
   using compose_programs_1 by blast
 
@@ -520,7 +467,7 @@ method dest_com_gen =
       in a[thin]: 
       "(init_while_cond;; 
                 WHILE _ \<noteq>0 DO (loop_body;; init_while_cond);;
-                after_loop, _) \<Rightarrow>\<^bsup>_\<^esup> _"
+                after_loop, _) \<Rightarrow>\<^sub>G\<^bsup>_\<^esup> _"
     for init_while_cond loop_body after_loop  \<Rightarrow> 
       \<open>match premises in b[thin]: "\<lbrakk>loop_cond; state_upd; _\<rbrakk> \<Longrightarrow> P"
        for loop_cond state_upd P \<Rightarrow> \<open>subst b[OF _ _ a]\<close>\<close>))
@@ -533,10 +480,42 @@ method dest_com_gen_time =
       in a[thin]: 
       "(init_while_cond;; 
                 WHILE _ \<noteq>0 DO (loop_body;; init_while_cond);;
-                after_loop, _) \<Rightarrow>\<^bsup>_\<^esup> _"
+                after_loop, _) \<Rightarrow>\<^sub>G\<^bsup>_\<^esup> _"
     for init_while_cond loop_body after_loop  \<Rightarrow> 
       \<open>match premises in b[thin]: "\<lbrakk>loop_cond; state_upd; _\<rbrakk> \<Longrightarrow> P"
        for loop_cond state_upd P \<Rightarrow> \<open>subst b[OF _ _ a, simplified add.assoc]\<close>\<close>))
 
+definition big_step_tG_concrete_cost :: "(com \<times> state \<Rightarrow> ('a \<Rightarrow> nat) \<Rightarrow> state \<Rightarrow> bool) \<Rightarrow> 'a \<Rightarrow> (com \<times> state \<Rightarrow> ('a \<Rightarrow> nat) \<Rightarrow> state \<Rightarrow> nat option)" where
+ "big_step_tG_concrete_cost bs x \<equiv> (\<lambda>cs C s. (if bs cs C s then Some (C x) else None))"
+
 end
+
+subsection "Naive Examples:"
+
+interpretation standard_fixed_costs : BS_Generalized_Cost
+  where skip_costs = "(\<lambda>x. (Suc 0))" and assign_costs = "(\<lambda>x. (Suc (Suc 0)))"
+  by (simp add: BS_Generalized_Cost.intro)
+
+(* Maybe it actually even makes sense*)
+fun naive_atomExp_costs :: "atomExp \<Rightarrow> nat" where
+ "naive_atomExp_costs (N n) = n + 1" |
+ "naive_atomExp_costs (V x) = 1"
+
+lemma naive_atomExp_costs_pos: "naive_atomExp_costs x > 0"
+  by (induction rule: naive_atomExp_costs.induct) auto
+
+fun variable_assign_costs :: "aexp \<Rightarrow> nat" where
+ "variable_assign_costs (A a) = Suc (Suc 0)" |
+ "variable_assign_costs (Plus a1 a2) = naive_atomExp_costs a1 + naive_atomExp_costs a2" |
+ "variable_assign_costs (Sub a1 a2) = naive_atomExp_costs a1 + naive_atomExp_costs a2" | 
+ "variable_assign_costs (Parity a) = naive_atomExp_costs a" |
+ "variable_assign_costs (RightShift a) = 2 ^ (naive_atomExp_costs a)"
+
+lemma variable_assign_costs_pos: " variable_assign_costs x > 0"
+  by (induction rule: variable_assign_costs.induct) (auto simp add: naive_atomExp_costs_pos)
+
+interpretation naive_variable_costs : BS_Generalized_Cost
+  where skip_costs = "(\<lambda>x. (Suc 0))" and assign_costs = "variable_assign_costs"
+  by (simp add: BS_Generalized_Cost.intro Suc_le_eq variable_assign_costs_pos)
+
 end
