IMP-/Step_Semantics_Cost_Generalization/Big_StepT_Generalized_Cost_Final.thy
@@ -1,6 +1,7 @@
-section "Big step semantics of IMP- generalized to include arbitrary* 
-         command cost functions"
-theory Big_StepT_Generalized_Cost imports Max_Constant Main Nat_Dom_Lifted Com "HOL-Eisbach.Eisbach_Tools" begin
+section "Big step semantics of IMP- generalized to include 
+         cost functions depending on command and arithmetic expression
+         loaded."
+theory Big_StepT_Generalized_Cost_Final imports "../Max_Constant" Main "../Com" "../Big_StepT" "HOL-Eisbach.Eisbach_Tools" begin
 
 paragraph "Summary"
 text\<open>We attempt to generalize big step semantics with time for IMP-. 
@@ -12,23 +13,36 @@ text "In IMP- Branching is only based on whether a variable's value equals 0."
 
 locale BS_Generalized_Cost =
   fixes skip_costs :: "state \<Rightarrow> nat" and 
-      assign_costs :: "aexp \<Rightarrow> state \<Rightarrow> nat"
-    assumes skip_cost_least: "\<And>x s s'. skip_costs s \<le> assign_costs x s'"
-    assumes assign_cost_positive: "\<And>x s. assign_costs x s > 0"
+      value_cost :: "nat \<Rightarrow> nat"
+    assumes skip_cost_pos: "\<And> s. skip_costs s > 0"
 begin 
 
-abbreviation "while_exit_costs \<equiv> (\<lambda>x. 2 * (skip_costs x))"
+
+
+fun atomVal_cost :: "atomExp \<Rightarrow> state \<Rightarrow> val" where
+"atomVal_cost (V var) s = value_cost (s var)"|
+"atomVal_cost (N number) _ = number"
+
+fun aexp_cost :: "aexp \<Rightarrow> state \<Rightarrow> nat" where 
+  "aexp_cost (A a) s = atomVal_cost a s" |
+  "aexp_cost (Plus a b) s = atomVal_cost a s + atomVal_cost b s" |
+  "aexp_cost (Sub a b) s = atomVal_cost a s + atomVal_cost b s" |
+  "aexp_cost (Parity n) s = atomVal_cost n s" |
+  "aexp_cost (RightShift n) s = atomVal_cost n s" 
+
+abbreviation "while_exit_costs \<equiv> (\<lambda>x. 1 + (skip_costs x))"
+abbreviation "assign_costs  \<equiv> (\<lambda>x y . aexp_cost x y + 1)"
 
 inductive
-  big_step_tG :: "com \<times> state \<Rightarrow> ('a \<Rightarrow> nat) \<Rightarrow> state \<Rightarrow> bool"  ("_ \<Rightarrow>\<^sub>G\<^bsup> _ \<^esup> _" 55)
+  big_step_tG :: "com \<times> state \<Rightarrow> nat \<Rightarrow> state \<Rightarrow> bool"  ("_ \<Rightarrow>\<^sub>G\<^bsup> _ \<^esup> _" 55)
 where
-Skip: "(SKIP,s) \<Rightarrow>\<^sub>G\<^bsup> skip_costs \<^esup> s"|
-Assign: "(x ::= a,s) \<Rightarrow>\<^sub>G\<^bsup> assign_costs \<^esup> s(x := aval a s)" |
-Seq: "\<lbrakk> (c1,s1) \<Rightarrow>\<^sub>G\<^bsup> C1 \<^esup> s2;  (c2,s2) \<Rightarrow>\<^sub>G\<^bsup> C2 \<^esup> s3 ; C3 = (\<lambda>x. (C1 x) + (C2 x)) \<rbrakk> \<Longrightarrow> (c1;;c2, s1) \<Rightarrow>\<^sub>G\<^bsup> C3 \<^esup> s3" |
-IfTrue: "\<lbrakk> s b \<noteq> 0;  (c1,s) \<Rightarrow>\<^sub>G\<^bsup> C \<^esup> t; C'= (\<lambda>x. (C x) + 1) \<rbrakk> \<Longrightarrow> (IF b \<noteq>0 THEN c1 ELSE c2, s) \<Rightarrow>\<^sub>G\<^bsup> C' \<^esup> t" |
-IfFalse: "\<lbrakk> s b = 0; (c2,s) \<Rightarrow>\<^sub>G\<^bsup> C \<^esup> t; C'= (\<lambda>x. (C x) + 1)  \<rbrakk> \<Longrightarrow> (IF b \<noteq>0 THEN c1 ELSE c2, s) \<Rightarrow>\<^sub>G\<^bsup> C' \<^esup> t" |
-WhileFalse: "\<lbrakk> s b = 0 \<rbrakk> \<Longrightarrow> (WHILE b \<noteq>0 DO c,s) \<Rightarrow>\<^sub>G\<^bsup> (\<lambda>x. 2 * (skip_costs x)) \<^esup> s" |
-WhileTrue: "\<lbrakk> s1 b \<noteq> 0;  (c,s1) \<Rightarrow>\<^sub>G\<^bsup> C1 \<^esup> s2;  (WHILE b \<noteq>0 DO c, s2) \<Rightarrow>\<^sub>G\<^bsup> C2 \<^esup> s3; C3 = (\<lambda>x. (C1 x) + (C2 x) + 1)\<rbrakk> 
+Skip: "(SKIP,s) \<Rightarrow>\<^sub>G\<^bsup> skip_costs s \<^esup> s"|
+Assign: "(x ::= a,s) \<Rightarrow>\<^sub>G\<^bsup> assign_costs a s \<^esup> s(x := aval a s)" |
+Seq: "\<lbrakk> (c1,s1) \<Rightarrow>\<^sub>G\<^bsup> C1 \<^esup> s2;  (c2,s2) \<Rightarrow>\<^sub>G\<^bsup> C2 \<^esup> s3 ; C3 = C1 + C2 \<rbrakk> \<Longrightarrow> (c1;;c2, s1) \<Rightarrow>\<^sub>G\<^bsup> C3 \<^esup> s3" |
+IfTrue: "\<lbrakk> s b \<noteq> 0;  (c1,s) \<Rightarrow>\<^sub>G\<^bsup> C \<^esup> t; C'= C + 1 \<rbrakk> \<Longrightarrow> (IF b \<noteq>0 THEN c1 ELSE c2, s) \<Rightarrow>\<^sub>G\<^bsup> C' \<^esup> t" |
+IfFalse: "\<lbrakk> s b = 0; (c2,s) \<Rightarrow>\<^sub>G\<^bsup> C \<^esup> t; C'=  C + 1 \<rbrakk> \<Longrightarrow> (IF b \<noteq>0 THEN c1 ELSE c2, s) \<Rightarrow>\<^sub>G\<^bsup> C' \<^esup> t" |
+WhileFalse: "\<lbrakk> s b = 0 \<rbrakk> \<Longrightarrow> (WHILE b \<noteq>0 DO c,s) \<Rightarrow>\<^sub>G\<^bsup> while_exit_costs s \<^esup> s" |
+WhileTrue: "\<lbrakk> s1 b \<noteq> 0;  (c,s1) \<Rightarrow>\<^sub>G\<^bsup> C1 \<^esup> s2;  (WHILE b \<noteq>0 DO c, s2) \<Rightarrow>\<^sub>G\<^bsup> C2 \<^esup> s3; C3 = C1 + C2 + 1\<rbrakk> 
     \<Longrightarrow> (WHILE b \<noteq>0 DO c, s1) \<Rightarrow>\<^sub>G\<^bsup> C3 \<^esup> s3" 
 end
 
@@ -71,6 +85,8 @@ end
 
 *)
 
+sledgehammer_params [provers = cvc4 verit z3 spass vampire zipperposition]
+
 context BS_Generalized_Cost begin
 
 subsection "proof automation:"
@@ -81,10 +97,8 @@ declare  BS_Generalized_Cost.big_step_tG.intros [intro]
 thm big_step_tG.induct
 
 text "Induction rules with pair splitting"
-lemmas big_step_tG_induct = big_step_tG.induct[split_format(complete), OF BS_Generalized_Cost_axioms]
-
-lemma "(c, s) \<Rightarrow>\<^sub>G\<^bsup> C \<^esup> s' \<Longrightarrow> BS_Generalized_Cost.big_step_tG skip_costs assign_costs (c, s) C s'"
-  by simp
+lemmas big_step_tG_induct = big_step_tG.induct[split_format(complete), 
+    OF BS_Generalized_Cost_axioms, consumes 1]
 
 subsection "Rule inversion"
 inductive_cases Skip_tE[elim!]: "(SKIP,s) \<Rightarrow>\<^sub>G\<^bsup> C \<^esup> t"
@@ -92,21 +106,21 @@ inductive_cases Assign_tE[elim!]: "(x ::= a,s) \<Rightarrow>\<^sub>G\<^bsup> C \
 inductive_cases Seq_tE[elim!]: "(c1;;c2,s1) \<Rightarrow>\<^sub>G\<^bsup> C \<^esup> s2"
 inductive_cases If_tE[elim!]: "(IF b \<noteq>0 THEN c1 ELSE c2,s) \<Rightarrow>\<^sub>G\<^bsup> C \<^esup> t"
 inductive_cases While_tE[elim]: "(WHILE b \<noteq>0 DO c,s) \<Rightarrow>\<^sub>G\<^bsup> C \<^esup> t"
-lemma Seq': "\<lbrakk>(c1,s1) \<Rightarrow>\<^sub>G\<^bsup> C1 \<^esup> s2;  (c2,s2) \<Rightarrow>\<^sub>G\<^bsup> C2 \<^esup> s3\<rbrakk> \<Longrightarrow> (c1;;c2, s1) \<Rightarrow>\<^sub>G\<^bsup> (\<lambda>x. C1 x + C2 x) \<^esup> s3"
+lemma Seq': "\<lbrakk>(c1,s1) \<Rightarrow>\<^sub>G\<^bsup> C1 \<^esup> s2;  (c2,s2) \<Rightarrow>\<^sub>G\<^bsup> C2 \<^esup> s3\<rbrakk> \<Longrightarrow> (c1;;c2, s1) \<Rightarrow>\<^sub>G\<^bsup> C1 + C2 \<^esup> s3"
   by (simp add: Seq)
 lemma While_tE': "\<lbrakk> s1 b \<noteq> 0;  (c,s1) \<Rightarrow>\<^sub>G\<^bsup> C1 \<^esup> s2;  (WHILE b \<noteq>0 DO c, s2) \<Rightarrow>\<^sub>G\<^bsup> C2 \<^esup> s3\<rbrakk> 
-    \<Longrightarrow> (WHILE b \<noteq>0 DO c, s1) \<Rightarrow>\<^sub>G\<^bsup> (\<lambda>x. (C1 x) + (C2 x) + 1) \<^esup> s3"
+    \<Longrightarrow> (WHILE b \<noteq>0 DO c, s1) \<Rightarrow>\<^sub>G\<^bsup> C1 + C2 + 1 \<^esup> s3"
   by (simp add: big_step_tG.WhileTrue)
 
 thm Seq_tE
 
 
-lemma Seq_costs_split: "(c1;;c2, s1) \<Rightarrow>\<^sub>G\<^bsup> C \<^esup> s3 \<Longrightarrow> \<exists>C1 C2 s2. ((c1,s1) \<Rightarrow>\<^sub>G\<^bsup> C1 \<^esup> s2) \<and>  ((c2,s2) \<Rightarrow>\<^sub>G\<^bsup> C2 \<^esup> s3) \<and> C = (\<lambda>x. (C1 x) + (C2 x))" 
+lemma Seq_costs_split: "(c1;;c2, s1) \<Rightarrow>\<^sub>G\<^bsup> C \<^esup> s3 \<Longrightarrow> \<exists>C1 C2 s2. ((c1,s1) \<Rightarrow>\<^sub>G\<^bsup> C1 \<^esup> s2) \<and>  ((c2,s2) \<Rightarrow>\<^sub>G\<^bsup> C2 \<^esup> s3) \<and> C = C1 + C2" 
   apply (erule Seq_tE)
   by auto
 
 lemma While_costs_split: "\<lbrakk> s1 b \<noteq> 0;  (WHILE b \<noteq>0 DO c, s1) \<Rightarrow>\<^sub>G\<^bsup> C \<^esup> s3\<rbrakk> 
-    \<Longrightarrow> \<exists>C1 C2 s2. ((c,s1) \<Rightarrow>\<^sub>G\<^bsup> C1 \<^esup> s2) \<and> ((WHILE b \<noteq>0 DO c, s2) \<Rightarrow>\<^sub>G\<^bsup> C2 \<^esup> s3) \<and> C = (\<lambda>x. (C1 x) + (C2 x) + 1)"
+    \<Longrightarrow> \<exists>C1 C2 s2. ((c,s1) \<Rightarrow>\<^sub>G\<^bsup> C1 \<^esup> s2) \<and> ((WHILE b \<noteq>0 DO c, s2) \<Rightarrow>\<^sub>G\<^bsup> C2 \<^esup> s3) \<and> C = C1 + C2  + 1"
   by force
 
 
@@ -121,12 +135,12 @@ lemma assumes "(IF b \<noteq>0 THEN SKIP ELSE SKIP, s) \<Rightarrow>\<^sub>G\<^b
   using assms apply cases by auto
 
 lemma assign_t_simp:
-  "((x ::= a,s) \<Rightarrow>\<^sub>G\<^bsup> assign_costs \<^esup>  s') \<longleftrightarrow> (s' = s(x := aval a s))"
+  "((x ::= a,s) \<Rightarrow>\<^sub>G\<^bsup> assign_costs a s\<^esup>  s') \<longleftrightarrow> (s' = s(x := aval a s))"
   using big_step_tG.Assign by auto
 
 lemma seq_costs_split: "(c1;;c2,s1) \<Rightarrow>\<^sub>G\<^bsup> C \<^esup> s2 \<Longrightarrow> 
                         \<exists>C1 C2 s. ((c1,s1) \<Rightarrow>\<^sub>G\<^bsup> C1 \<^esup> s) \<and> ((c2,s) \<Rightarrow>\<^sub>G\<^bsup> C2 \<^esup> s2)
-                        \<and> C = (\<lambda>x. (C1 x) + (C2 x)) " by auto
+                        \<and> C = C1 + C2 " by auto
 
 subsection "Determinism of Big semantics of IMP-"
 theorem big_step_t_state_determ2: "\<lbrakk> (c,s) \<Rightarrow>\<^sub>G\<^bsup> p \<^esup> t; (c,s) \<Rightarrow>\<^sub>G\<^bsup> q \<^esup> u \<rbrakk> \<Longrightarrow> (u = t)"
@@ -185,32 +199,32 @@ next
     by auto
 next
   case (WhileTrue s1 b c C1 s2 C2 s3 C3)
-  then show ?case  proof-
+  then show ?case proof-
     obtain q1 q2 s2' where "
    ((c, s1) \<Rightarrow>\<^sub>G\<^bsup> q1 \<^esup> s2') \<and>
-   ((WHILE b\<noteq>0 DO c, s2') \<Rightarrow>\<^sub>G\<^bsup> q2 \<^esup> s3) \<and> q = (\<lambda>x. q1 x + q2 x + 1)"
+   ((WHILE b\<noteq>0 DO c, s2') \<Rightarrow>\<^sub>G\<^bsup> q2 \<^esup> s3) \<and> q = q1 + q2 + 1"
       using WhileTrue.hyps(1) WhileTrue.prems by auto
     have "s2' = s2" 
-      using WhileTrue.hyps(2) \<open>((c, s1) \<Rightarrow>\<^sub>G\<^bsup> q1 \<^esup> s2') \<and> ((WHILE b\<noteq>0 DO c, s2') \<Rightarrow>\<^sub>G\<^bsup> q2 \<^esup> s3) \<and> q = (\<lambda>x. q1 x + q2 x + 1)\<close> big_step_t_state_determ2 by auto
+      using WhileTrue.hyps(2) \<open>((c, s1) \<Rightarrow>\<^sub>G\<^bsup> q1 \<^esup> s2') \<and> ((WHILE b\<noteq>0 DO c, s2') \<Rightarrow>\<^sub>G\<^bsup> q2 \<^esup> s3) \<and> q = ( q1 + q2 + 1)\<close> big_step_t_state_determ2 by auto
     moreover have "q1 = C1"
     proof- have "(c, s1) \<Rightarrow>\<^sub>G\<^bsup> q1 \<^esup> s2" 
-        using \<open>((c, s1) \<Rightarrow>\<^sub>G\<^bsup> q1 \<^esup> s2') \<and> ((WHILE b\<noteq>0 DO c, s2') \<Rightarrow>\<^sub>G\<^bsup> q2 \<^esup> s3) \<and> q = (\<lambda>x. q1 x + q2 x + 1)\<close> calculation by auto
+        using \<open>((c, s1) \<Rightarrow>\<^sub>G\<^bsup> q1 \<^esup> s2') \<and> ((WHILE b\<noteq>0 DO c, s2') \<Rightarrow>\<^sub>G\<^bsup> q2 \<^esup> s3) \<and> q = ( q1  + q2  + 1)\<close> calculation by auto
       thus ?thesis 
         using WhileTrue.IH(1) by auto
     qed
     moreover have "q2 = C2"
     proof- have "(WHILE b\<noteq>0 DO c, s2) \<Rightarrow>\<^sub>G\<^bsup> q2 \<^esup> s3" 
         using \<open>((c, s1) \<Rightarrow>\<^sub>G\<^bsup> q1 \<^esup> s2') \<and>
-   ((WHILE b\<noteq>0 DO c, s2') \<Rightarrow>\<^sub>G\<^bsup> q2 \<^esup> s3) \<and> q = (\<lambda>x. q1 x + q2 x + 1)\<close> calculation by auto
+   ((WHILE b\<noteq>0 DO c, s2') \<Rightarrow>\<^sub>G\<^bsup> q2 \<^esup> s3) \<and> q = (q1 + q2 + 1)\<close> calculation by auto
       thus ?thesis 
         by (simp add: WhileTrue.IH(2))
     qed
-    moreover have "q = (\<lambda>x. C1 x + C2 x + 1)" 
+    moreover have "q = (C1 + C2 + 1)" 
     proof-
-      have " q = (\<lambda>x. q1 x + q2 x + 1)" using \<open>((c, s1) \<Rightarrow>\<^sub>G\<^bsup> q1 \<^esup> s2') \<and> ((WHILE b\<noteq>0 DO c, s2') \<Rightarrow>\<^sub>G\<^bsup> q2 \<^esup> s3) \<and> q = (\<lambda>x. q1 x + q2 x + 1)\<close>
+      have " q = (q1 + q2 + 1)" using \<open>((c, s1) \<Rightarrow>\<^sub>G\<^bsup> q1 \<^esup> s2') \<and> ((WHILE b\<noteq>0 DO c, s2') \<Rightarrow>\<^sub>G\<^bsup> q2 \<^esup> s3) \<and> q = (q1 + q2 + 1)\<close>
         by simp
       thus ?thesis using calculation(2-3)
-        by (simp add: \<open>q = (\<lambda>x. q1 x + q2 x + 1)\<close>)
+        by (simp add: \<open>q = (q1 + q2 + 1)\<close>)
     qed
     ultimately show ?thesis 
       by (simp add: WhileTrue.hyps(4))
@@ -222,73 +236,60 @@ lemma bigstep_det: "(c1, s) \<Rightarrow>\<^sub>G\<^bsup> p1 \<^esup> t1 \<Longr
 
 
 lemma seq_assign_t_simp:
-  "((c ;; x ::= a, s) \<Rightarrow>\<^sub>G\<^bsup> (\<lambda>x. t x + assign_costs x) \<^esup>  s') 
-  \<longleftrightarrow> (\<exists>s''. ((c, s) \<Rightarrow>\<^sub>G\<^bsup> t \<^esup> s'') \<and> s' = s''(x := aval a s''))"
+  "((c ;; x ::= a, s) \<Rightarrow>\<^sub>G\<^bsup> t \<^esup>  s') 
+  \<longleftrightarrow> (\<exists>s'' t'. t = t' + assign_costs a s'' \<and> ((c, s) \<Rightarrow>\<^sub>G\<^bsup> t' \<^esup> s'') \<and> s' = s''(x := aval a s''))"
 proof
-  assume "(c;; x ::= a, s) \<Rightarrow>\<^sub>G\<^bsup> (\<lambda>x. t x + assign_costs x) \<^esup> s'"
+  assume "(c;; x ::= a, s) \<Rightarrow>\<^sub>G\<^bsup> t \<^esup> s'"
   thm seq_costs_split
-  then obtain C1 C2 s'' where "(c, s) \<Rightarrow>\<^sub>G\<^bsup> C1 \<^esup> s''" 
-                          and "(x ::= a, s'') \<Rightarrow>\<^sub>G\<^bsup> C2 \<^esup> s'" 
-                          and " (\<lambda>x. t x + assign_costs x) = (\<lambda>x. C1 x + C2 x)"
-    using \<open>(c;; x ::= a, s) \<Rightarrow>\<^sub>G\<^bsup> (\<lambda>x. t x + assign_costs x) \<^esup> s'\<close> seq_costs_split 
-    by meson
-  have "assign_costs = C2" using \<open>(c;; x ::= a, s) \<Rightarrow>\<^sub>G\<^bsup>  (\<lambda>x. t x + assign_costs x) \<^esup> s'\<close>
-    using \<open>(x ::= a, s'') \<Rightarrow>\<^sub>G\<^bsup> C2 \<^esup> s'\<close> by auto
-  hence "(\<lambda>x. t x + assign_costs x) = (\<lambda>x. C1 x + assign_costs x)" 
-    using \<open>(\<lambda>x. t x + assign_costs x) = (\<lambda>x. C1 x + C2 x)\<close> by auto 
-  hence "t = C1" using add_right_cancel_lifted by auto
-  thus "\<exists>s''. ((c, s) \<Rightarrow>\<^sub>G\<^bsup> t \<^esup> s'') \<and> s' = s''(x := aval a s'')"
-    using \<open>(c, s) \<Rightarrow>\<^sub>G\<^bsup> C1 \<^esup> s''\<close> \<open>(x ::= a, s'') \<Rightarrow>\<^sub>G\<^bsup> C2 \<^esup> s'\<close> by auto
+  then obtain t' s'' where "(c, s) \<Rightarrow>\<^sub>G\<^bsup> t' \<^esup> s''" 
+                          and "(x ::= a, s'') \<Rightarrow>\<^sub>G\<^bsup> assign_costs a s'' \<^esup> s'" 
+                          and "t = t' + assign_costs a s''"
+    using local.assign_t_simp by force
+  moreover have "\<exists>s'' t'. ((c, s) \<Rightarrow>\<^sub>G\<^bsup> t' \<^esup> s'') \<and> s' = s''(x := aval a s'')"
+    using \<open>(c, s) \<Rightarrow>\<^sub>G\<^bsup> t' \<^esup> s''\<close> \<open>(x ::= a, s'') \<Rightarrow>\<^sub>G\<^bsup> assign_costs a s'' \<^esup> s'\<close> by auto
+  ultimately show "\<exists>s'' t'. t = t' + assign_costs a s'' \<and> ((c, s) \<Rightarrow>\<^sub>G\<^bsup> t' \<^esup> s'') \<and> s' = s''(x := aval a s'')"
+    by blast
 next
-  assume "\<exists>s''. ((c, s) \<Rightarrow>\<^sub>G\<^bsup> t \<^esup> s'') \<and> s' = s''(x := aval a s'')"
-  thus "(c ;; x ::= a, s) \<Rightarrow>\<^sub>G\<^bsup> (\<lambda>x. t x + assign_costs x) \<^esup>  s'"
-    using Seq' big_step_tG.Assign by auto
+  assume "\<exists>s'' t'. t = t' + assign_costs a s'' \<and> ((c, s) \<Rightarrow>\<^sub>G\<^bsup> t' \<^esup> s'') \<and> s' = s''(x := aval a s'')"
+  show "(c ;; x ::= a, s) \<Rightarrow>\<^sub>G\<^bsup> t \<^esup>  s'"
+    using BS_Generalized_Cost_axioms \<open>\<exists>s'' t'. t = t' + assign_costs a s'' \<and> (c, s) \<Rightarrow>\<^sub>G\<^bsup> t' \<^esup> s'' \<and> s' = s''(x := aval a s'')\<close> by auto
 qed 
 
-lemma seq_assign_t_intro: "(c, s) \<Rightarrow>\<^sub>G\<^bsup> t \<^esup> s'' \<Longrightarrow> s' = s''(x := aval a s'')
-  \<Longrightarrow>(c ;; x ::= a, s) \<Rightarrow>\<^sub>G\<^bsup> (\<lambda>x. t x + assign_costs x) \<^esup>  s'"
-  using seq_assign_t_simp 
-  by auto
-
-lemma seq_is_noop[simp]: "((SKIP, s) \<Rightarrow>\<^sub>G\<^bsup>t\<^esup> s') \<longleftrightarrow> (t = skip_costs \<and> s = s')" 
+lemma seq_is_noop[simp]: "((SKIP, s) \<Rightarrow>\<^sub>G\<^bsup>t\<^esup> s') \<longleftrightarrow> (t = skip_costs s \<and> s = s')" 
   using Skip by auto
 
-lemma seq_skip[simp]: "((c ;; SKIP, s) \<Rightarrow>\<^sub>G\<^bsup>(\<lambda>x. t x + skip_costs x)\<^esup> s') \<longleftrightarrow> ((c, s) \<Rightarrow>\<^sub>G\<^bsup>t\<^esup> s')"
-  apply auto 
-  apply (simp add: add_right_cancel_lifted)
-  by (simp add: Seq')
+lemma seq_skip[simp]: "((c ;; SKIP, s) \<Rightarrow>\<^sub>G\<^bsup> t + skip_costs s'\<^esup> s') \<longleftrightarrow> ((c, s) \<Rightarrow>\<^sub>G\<^bsup>t\<^esup> s')"
+  by (auto simp add: Seq')
 
 subsection "Progress property"
 text "every command costs time"
 
-(* Needs extra skip assumption to hold, not sure if we want it for the general case *)
-
-lemma bigstep_progress:  "(c, s) \<Rightarrow>\<^sub>G\<^bsup> p \<^esup> t \<Longrightarrow> \<forall>x. skip_costs x > 0 \<Longrightarrow>  \<forall>x. p x > 0"
+lemma bigstep_progress:  "(c, s) \<Rightarrow>\<^sub>G\<^bsup> p \<^esup> t \<Longrightarrow> p > 0"
   apply(induct rule: big_step_tG.induct, auto)
-  by (simp add: assign_cost_positive)
-
+  by (simp add: skip_cost_pos)
+  
 subsection "abbreviations and properties"
-abbreviation terminates ("\<down>") where "terminates cs \<equiv> (\<exists>n a. (cs \<Rightarrow>\<^sub>G\<^bsup> n \<^esup> a))"
-abbreviation thestate ("\<down>\<^sub>s") where "thestate cs \<equiv> (THE a. \<exists>n. (cs \<Rightarrow>\<^sub>G\<^bsup> n \<^esup> a))" 
-abbreviation thetime ("\<down>\<^sub>t") where "thetime cs \<equiv> (THE n. \<exists>a. (cs \<Rightarrow>\<^sub>G\<^bsup> n \<^esup> a))"
+abbreviation terminates ("\<down>\<^sub>G") where "terminates cs \<equiv> (\<exists>n a. (cs \<Rightarrow>\<^sub>G\<^bsup> n \<^esup> a))"
+abbreviation thestate ("\<down>\<^sub>G\<^sub>s") where "thestate cs \<equiv> (THE a. \<exists>n. (cs \<Rightarrow>\<^sub>G\<^bsup> n \<^esup> a))" 
+abbreviation thetime ("\<down>\<^sub>G\<^sub>t") where "thetime cs \<equiv> (THE n. \<exists>a. (cs \<Rightarrow>\<^sub>G\<^bsup> n \<^esup> a))"
 
-lemma bigstepT_the_cost: "(c, s) \<Rightarrow>\<^sub>G\<^bsup> t \<^esup> s' \<Longrightarrow> \<down>\<^sub>t(c, s) = t"
+lemma bigstepT_the_cost: "(c, s) \<Rightarrow>\<^sub>G\<^bsup> t \<^esup> s' \<Longrightarrow> \<down>\<^sub>G\<^sub>t(c, s) = t"
   using bigstep_det by blast 
 
-lemma bigstepT_the_state: "(c, s) \<Rightarrow>\<^sub>G\<^bsup> t \<^esup> s' \<Longrightarrow> \<down>\<^sub>s(c, s) = s'"
+lemma bigstepT_the_state: "(c, s) \<Rightarrow>\<^sub>G\<^bsup> t \<^esup> s' \<Longrightarrow> \<down>\<^sub>G\<^sub>s(c, s) = s'"
   using bigstep_det by blast 
 
-lemma SKIPnot: "(\<not> ((SKIP, s) \<Rightarrow>\<^sub>G\<^bsup> p \<^esup> t)) \<longleftrightarrow> (s\<noteq>t \<or> p\<noteq>skip_costs)" by auto
+lemma SKIPnot: "(\<not> ((SKIP, s) \<Rightarrow>\<^sub>G\<^bsup> p \<^esup> t)) \<longleftrightarrow> (s\<noteq>t \<or> p\<noteq>skip_costs s)" by auto
 
-lemma SKIPp: "\<down>\<^sub>t(SKIP,s) = skip_costs"
+lemma SKIPp: "\<down>\<^sub>G\<^sub>t(SKIP,s) = skip_costs s"
   apply(rule the_equality)
   apply auto done 
 
-lemma SKIPt: "\<down>\<^sub>s(SKIP,s) = s"
+lemma SKIPt: "\<down>\<^sub>G\<^sub>s(SKIP,s) = s"
   apply(rule the_equality)
   apply auto done 
 
-lemma ASSp: "(THE p. Ex (big_step_tG (x ::= e, s) p)) = assign_costs"
+lemma ASSp: "(THE p. Ex (big_step_tG (x ::= e, s) p)) = assign_costs e s"
   apply(rule the_equality)
   apply auto 
   using big_step_tG.Assign by auto  
@@ -298,9 +299,9 @@ lemma ASSt: "(THE t. \<exists>p. ((x ::= e, s) \<Rightarrow>\<^sub>G\<^bsup> p \
   apply auto 
   using big_step_tG.Assign by auto
 
-lemma ASSnot: "( \<not>((x ::= e, s) \<Rightarrow>\<^sub>G\<^bsup> p \<^esup> t )) = (p\<noteq>assign_costs \<or> t\<noteq>s(x := aval e s))"
+lemma ASSnot: "( \<not>((x ::= e, s) \<Rightarrow>\<^sub>G\<^bsup> p \<^esup> t )) = (p\<noteq>assign_costs e s \<or> t\<noteq>s(x := aval e s))"
   apply auto
-  by (simp add: big_step_tG.Assign)
+  using big_step_tG.Assign by auto
 
 (*
 lemma If_THE_True: "Suc (THE n. \<exists>a. (c1, s) \<Rightarrow>\<^sub>G\<^bsup> n \<^esup> a) =  (THE n. \<exists>a. (IF b \<noteq>0 THEN c1 ELSE c2, s) \<Rightarrow>\<^sub>G\<^bsup> n \<^esup> a)"
@@ -365,22 +366,22 @@ lemma terminates_split_if : "(P s \<Longrightarrow> (c, s) \<Rightarrow>\<^sub>G
   by auto
 
 lemma AssignD': 
-"(x ::= a, s) \<Rightarrow>\<^sub>G\<^bsup> assign_costs \<^esup> s' \<Longrightarrow> s' = s (x:= aval a s)"
+"(x ::= a, s) \<Rightarrow>\<^sub>G\<^bsup> assign_costs a s\<^esup> s' \<Longrightarrow> s' = s (x:= aval a s)"
   by (auto simp add: eval_nat_numeral)
 
 (* TODO: Probably needs induction with pairs, needs fixing *)
 lemma com_only_vars: "\<lbrakk>(c, s) \<Rightarrow>\<^sub>G\<^bsup> t \<^esup> s'; x \<notin> set (Max_Constant.all_variables c)\<rbrakk> \<Longrightarrow> s x = s' x"
-  apply (induction arbitrary: x rule: big_step_tG.induct) 
-  oops
+  apply (induction c s t s' arbitrary: x rule: big_step_tG_induct) 
+  sorry
 
 lemma Seq'': "\<lbrakk> ((c1,s1) \<Rightarrow>\<^sub>G\<^bsup> x \<^esup> s2) \<and> P s2; P s2 \<Longrightarrow> ((c2,s2) \<Rightarrow>\<^sub>G\<^bsup> y \<^esup> s3) \<and> Q s3; Q s3 \<Longrightarrow> R s3 \<rbrakk>
-             \<Longrightarrow> ((c1;;c2, s1) \<Rightarrow>\<^sub>G\<^bsup> (\<lambda>z. (x z) + (y z))\<^esup> s3) \<and> R s3"
+             \<Longrightarrow> ((c1;;c2, s1) \<Rightarrow>\<^sub>G\<^bsup> x + y \<^esup> s3) \<and> R s3"
   apply auto by (simp add: Seq')
 
 lemma WhileI:
 "\<lbrakk>(s1 b \<noteq> 0 \<Longrightarrow> ((c,s1) \<Rightarrow>\<^sub>G\<^bsup> x \<^esup> s2) \<and> ((WHILE b \<noteq>0 DO c, s2) \<Rightarrow>\<^sub>G\<^bsup> y \<^esup> s3));
   (s1 b = 0 \<Longrightarrow> s1 = s3);
-  z = (if s1 b \<noteq> 0 then (\<lambda>z. (x z) + (y z) + 1) else (\<lambda>x. 2 * (skip_costs x)))\<rbrakk>
+  z = (if s1 b \<noteq> 0 then (x + y + 1) else while_exit_costs s1)\<rbrakk>
         \<Longrightarrow> (WHILE b \<noteq>0 DO c, s1) \<Rightarrow>\<^sub>G\<^bsup> z \<^esup> s3" 
   using WhileTrue 
    apply auto[1]
@@ -390,7 +391,7 @@ lemma WhileI:
 lemma IfI:
 "\<lbrakk>s b \<noteq> 0 \<Longrightarrow> (c1,s) \<Rightarrow>\<^sub>G\<^bsup> x1 \<^esup> t1;
   s b = 0 \<Longrightarrow> (c2,s) \<Rightarrow>\<^sub>G\<^bsup> x2 \<^esup> t2;
-  y = (\<lambda>x. (if s b \<noteq> 0 then x1 else x2) x + 1);
+  y = ((if s b \<noteq> 0 then x1 else x2) + 1);
   t = (if s b \<noteq> 0 then t1 else t2)\<rbrakk>
         \<Longrightarrow> (IF b \<noteq>0 THEN c1 ELSE c2, s) \<Rightarrow>\<^sub>G\<^bsup> y \<^esup> t" 
   by (auto simp add: IfTrue IfFalse)
@@ -398,65 +399,61 @@ lemma IfI:
 thm Suc_inject
 
 lemma IfE: 
-"(IF b \<noteq>0 THEN c1 ELSE c2, s) \<Rightarrow>\<^sub>G\<^bsup> (\<lambda>x. (if s b \<noteq> 0 then x1 else x2) x + 1) \<^esup> (if s b \<noteq> 0 then s1 else s2) \<Longrightarrow> 
- \<lbrakk>\<lbrakk>s b \<noteq> 0; (\<lambda>x. (if s b \<noteq> 0 then x1 else x2) x + 1) = (\<lambda>x. x1 x + 1); 
+"(IF b \<noteq>0 THEN c1 ELSE c2, s) \<Rightarrow>\<^sub>G\<^bsup> ((if s b \<noteq> 0 then x1 else x2) + 1) \<^esup> (if s b \<noteq> 0 then s1 else s2) \<Longrightarrow> 
+ \<lbrakk>\<lbrakk>s b \<noteq> 0; ((if s b \<noteq> 0 then x1 else x2) + 1) = (x1 + 1); 
   (if s b \<noteq> 0 then s1 else s2) = s1; (c1,s) \<Rightarrow>\<^sub>G\<^bsup> x1 \<^esup> s1\<rbrakk> \<Longrightarrow> P;
-  \<lbrakk>s b = 0; (\<lambda>x. (if s b \<noteq> 0 then x1 else x2) x + 1) = (\<lambda>x. x2 x + 1);
+  \<lbrakk>s b = 0; ((if s b \<noteq> 0 then x1 else x2) + 1) = x2 + 1;
    (if s b \<noteq> 0 then s1 else s2) = s2; (c2,s) \<Rightarrow>\<^sub>G\<^bsup> x2 \<^esup> s2\<rbrakk> \<Longrightarrow> P\<rbrakk>
         \<Longrightarrow> P"
-  apply (auto simp add: IfTrue IfFalse) 
-   apply (metis add_right_cancel_lifted old.nat.inject)
-  by (metis add_right_cancel_lifted nat.inject)
+  by (auto simp add: IfTrue IfFalse) 
 thm Seq_tE
 
 lemma IfD:
-"(IF b \<noteq>0 THEN c1 ELSE c2, s) \<Rightarrow>\<^sub>G\<^bsup> (\<lambda>x. (if s b \<noteq> 0 then x1 else x2) x + 1) \<^esup> (if s b \<noteq> 0 then t1 else t2) \<Longrightarrow> 
+"(IF b \<noteq>0 THEN c1 ELSE c2, s) \<Rightarrow>\<^sub>G\<^bsup> (if s b \<noteq> 0 then x1 else x2) + 1 \<^esup> (if s b \<noteq> 0 then t1 else t2) \<Longrightarrow> 
  \<lbrakk>\<lbrakk>s b \<noteq> 0; (c1,s) \<Rightarrow>\<^sub>G\<^bsup> x1 \<^esup> t1\<rbrakk> \<Longrightarrow> P;
   \<lbrakk>s b = 0; (c2,s) \<Rightarrow>\<^sub>G\<^bsup> x2 \<^esup> t2\<rbrakk> \<Longrightarrow> P\<rbrakk>
         \<Longrightarrow> P" 
-  apply (auto simp add: IfTrue IfFalse)
-   apply (metis add_right_cancel_lifted old.nat.inject) 
-  by (metis add_right_cancel_lifted nat.inject)
+  by (auto simp add: IfTrue IfFalse)
 
 lemma AssignI:
 "\<lbrakk>s' = s (x:= aval a s)\<rbrakk>
-        \<Longrightarrow> (x ::= a, s) \<Rightarrow>\<^sub>G\<^bsup> assign_costs \<^esup> s'" 
-  by (auto simp add: Assign)
+        \<Longrightarrow> (x ::= a, s) \<Rightarrow>\<^sub>G\<^bsup> assign_costs a s\<^esup> s'" 
+  using big_step_tG.Assign by auto
 
 lemma AssignI': 
 "\<lbrakk>s' = s (x:= aval a s)\<rbrakk>
-        \<Longrightarrow> (x ::= a, s) \<Rightarrow>\<^sub>G\<^bsup> assign_costs \<^esup> s'" 
-  by (auto simp add: Assign eval_nat_numeral)
+        \<Longrightarrow> (x ::= a, s) \<Rightarrow>\<^sub>G\<^bsup> assign_costs a s\<^esup> s'" 
+  using big_step_tG.Assign by auto
 
 lemma AssignI'': 
 "\<lbrakk>s' = s (x:= aval a s)\<rbrakk>
-        \<Longrightarrow> ((x ::= a, s) \<Rightarrow>\<^sub>G\<^bsup> assign_costs \<^esup> s') \<and> (s' = s')" 
-  by (auto simp add: Assign eval_nat_numeral)
+        \<Longrightarrow> ((x ::= a, s) \<Rightarrow>\<^sub>G\<^bsup> assign_costs a s\<^esup> s') \<and> (s' = s')" 
+  using big_step_tG.Assign by auto
 
-lemma AssignD: "(x ::= a, s) \<Rightarrow>\<^sub>G\<^bsup> t \<^esup> s' \<Longrightarrow> t = assign_costs \<and> s' = s(x := aval a s)"
+lemma AssignD: "(x ::= a, s) \<Rightarrow>\<^sub>G\<^bsup> t \<^esup> s' \<Longrightarrow> t = assign_costs a s \<and> s' = s(x := aval a s)"
   by auto
 
 lemma compose_programs_1:
   "(c2, s2) \<Rightarrow>\<^sub>G\<^bsup> y \<^esup> s3 \<Longrightarrow> (c1, s1) \<Rightarrow>\<^sub>G\<^bsup> x \<^esup> s2 \<Longrightarrow> 
-    ((c1;; c2, s1) \<Rightarrow>\<^sub>G\<^bsup> (\<lambda>z. x z + y z) \<^esup> s3 \<Longrightarrow> P)
+    ((c1;; c2, s1) \<Rightarrow>\<^sub>G\<^bsup>x + y\<^esup> s3 \<Longrightarrow> P)
    \<Longrightarrow> P" 
   by (simp add: Seq')
 
 lemma compose_programs_2:
   "(c1, s1) \<Rightarrow>\<^sub>G\<^bsup> x \<^esup> s2 \<Longrightarrow> (c2, s2) \<Rightarrow>\<^sub>G\<^bsup> y \<^esup> s3 \<Longrightarrow> 
-    ((c1;; c2, s1) \<Rightarrow>\<^sub>G\<^bsup> (\<lambda>z. x z + y z) \<^esup> s3 \<Longrightarrow> P)
+    ((c1;; c2, s1) \<Rightarrow>\<^sub>G\<^bsup>x + y\<^esup> s3 \<Longrightarrow> P)
    \<Longrightarrow> P"
   by (simp add: Seq')
 
 lemma While_tE_time:
 "(WHILE b\<noteq>0 DO c, s) \<Rightarrow>\<^sub>G\<^bsup> x \<^esup> t \<Longrightarrow>
-  (x = (\<lambda>x. 2 * (skip_costs x)) \<Longrightarrow> t = s \<Longrightarrow> s b = 0 \<Longrightarrow> P) \<Longrightarrow>
-  (\<And>x' s2 y. 0 < s b \<Longrightarrow> (c, s) \<Rightarrow>\<^sub>G\<^bsup> x' \<^esup> s2 \<Longrightarrow> (WHILE b\<noteq>0 DO c, s2) \<Rightarrow>\<^sub>G\<^bsup> y \<^esup> t \<Longrightarrow> x = (\<lambda>z. x' z + y z + 1) \<Longrightarrow> P) \<Longrightarrow> P"
+  (x = while_exit_costs s \<Longrightarrow> t = s \<Longrightarrow> s b = 0 \<Longrightarrow> P) \<Longrightarrow>
+  (\<And>x' s2 y. 0 < s b \<Longrightarrow> (c, s) \<Rightarrow>\<^sub>G\<^bsup> x' \<^esup> s2 \<Longrightarrow> (WHILE b\<noteq>0 DO c, s2) \<Rightarrow>\<^sub>G\<^bsup> y \<^esup> t \<Longrightarrow> x = (x' + y  + 1) \<Longrightarrow> P) \<Longrightarrow> P"
   by auto
 
 lemma Seq_tE_While_init:
   "(WHILE v \<noteq>0 DO c2, s2) \<Rightarrow>\<^sub>G\<^bsup> y \<^esup> s3 \<Longrightarrow> (c1, s1) \<Rightarrow>\<^sub>G\<^bsup> x \<^esup> s2 \<Longrightarrow> 
-    ((c1;; WHILE v \<noteq>0 DO c2, s1) \<Rightarrow>\<^sub>G\<^bsup> (\<lambda>z. x z + y z) \<^esup> s3 \<Longrightarrow> P)
+    ((c1;; WHILE v \<noteq>0 DO c2, s1) \<Rightarrow>\<^sub>G\<^bsup> x + y \<^esup> s3 \<Longrightarrow> P)
    \<Longrightarrow> P"
   using compose_programs_1 by blast
 
@@ -489,33 +486,5 @@ definition big_step_tG_concrete_cost :: "(com \<times> state \<Rightarrow> ('a \
  "big_step_tG_concrete_cost bs x \<equiv> (\<lambda>cs C s. (if bs cs C s then Some (C x) else None))"
 
 end
-
-subsection "Naive Examples:"
-
-interpretation standard_fixed_costs : BS_Generalized_Cost
-  where skip_costs = "(\<lambda>x. (Suc 0))" and assign_costs = "(\<lambda>x. (Suc (Suc 0)))"
-  by (simp add: BS_Generalized_Cost.intro)
-
-(* Maybe it actually even makes sense*)
-fun naive_atomExp_costs :: "atomExp \<Rightarrow> nat" where
- "naive_atomExp_costs (N n) = n + 1" |
- "naive_atomExp_costs (V x) = 1"
-
-lemma naive_atomExp_costs_pos: "naive_atomExp_costs x > 0"
-  by (induction rule: naive_atomExp_costs.induct) auto
-
-fun variable_assign_costs :: "aexp \<Rightarrow> nat" where
- "variable_assign_costs (A a) = Suc (Suc 0)" |
- "variable_assign_costs (Plus a1 a2) = naive_atomExp_costs a1 + naive_atomExp_costs a2" |
- "variable_assign_costs (Sub a1 a2) = naive_atomExp_costs a1 + naive_atomExp_costs a2" | 
- "variable_assign_costs (Parity a) = naive_atomExp_costs a" |
- "variable_assign_costs (RightShift a) = 2 ^ (naive_atomExp_costs a)"
-
-lemma variable_assign_costs_pos: " variable_assign_costs x > 0"
-  by (induction rule: variable_assign_costs.induct) (auto simp add: naive_atomExp_costs_pos)
-
-interpretation naive_variable_costs : BS_Generalized_Cost
-  where skip_costs = "(\<lambda>x. (Suc 0))" and assign_costs = "variable_assign_costs"
-  by (simp add: BS_Generalized_Cost.intro Suc_le_eq variable_assign_costs_pos)
 
 end
