IMP-/Step_Semantics_Cost_Generalization/Nat_Dom_Lifted.thy
@@ -1,7 +1,0 @@
-theory Nat_Dom_Lifted
-  imports  "../AExp" "~~/src/HOL/Library/Simps_Case_Conv"
-begin
-
-
-
-end
