IMP-/Step_Semantics_Cost_Generalization/Vars_for_GC.thy
@@ -1,0 +1,442 @@
+theory Vars_for_GC imports Big_StepT_Generalized_Cost_Final "../Eq_On"
+begin
+
+
+
+sledgehammer_params [provers = cvc4 verit z3 spass vampire zipperposition]
+
+class vars =
+  fixes vars :: "'a \<Rightarrow> vname list"
+
+class subst = vars +
+  fixes subst :: "(vname \<Rightarrow> vname) \<Rightarrow> 'a \<Rightarrow> 'a"
+  assumes subst_vars[simp]: "set (vars (subst m c)) = m ` set (vars c)"
+
+instantiation atomExp :: vars
+begin
+
+fun vars_atomExp :: "atomExp \<Rightarrow> vname list" where
+"vars_atomExp (V var) = [var]" |
+"vars_atomExp (N _) = []"
+
+instance ..
+
+end
+
+instantiation atomExp :: subst
+begin
+
+fun subst_atomExp :: "(vname \<Rightarrow> vname) \<Rightarrow> atomExp \<Rightarrow> atomExp" where
+"subst m (V var) = V (m var)" |
+"subst m (N n) = N n"
+
+instance
+proof (standard, goal_cases)
+  case (1 m c)
+  then show ?case by (induction c) auto
+qed
+
+end
+
+instantiation aexp :: vars
+begin
+
+fun vars_aexp :: "aexp \<Rightarrow> vname list" where
+"vars (A e) = vars e" |
+"vars (Plus e\<^sub>1 e\<^sub>2) = vars e\<^sub>1 @ vars e\<^sub>2" |
+"vars (Sub e\<^sub>1 e\<^sub>2) = vars e\<^sub>1 @ vars e\<^sub>2" |
+"vars (Parity e) = vars e" |
+"vars (RightShift e) = vars e"
+
+instance ..
+
+end
+
+instantiation aexp :: subst
+begin
+
+fun subst_aexp :: "(vname \<Rightarrow> vname) \<Rightarrow> aexp \<Rightarrow> aexp" where
+"subst m (A e) = A (subst m e)" |
+"subst m (Plus e\<^sub>1 e\<^sub>2) = Plus (subst m e\<^sub>1) (subst m e\<^sub>2)" |
+"subst m (Sub e\<^sub>1 e\<^sub>2) = Sub (subst m e\<^sub>1) (subst m e\<^sub>2)" |
+"subst m (Parity e) = Parity (subst m e)" |
+"subst m (RightShift e) = RightShift (subst m e)"
+
+instance
+proof (standard, goal_cases)
+  case (1 m c)
+  then show ?case by (induction c) auto
+qed
+
+end
+
+
+lemma atomVal_eq_if_eq_on_vars[simp]:
+  "s\<^sub>1 = s\<^sub>2 on set (vars a) \<Longrightarrow> atomVal a s\<^sub>1 = atomVal a s\<^sub>2"
+  by (induction a) auto
+
+lemma aval_eq_if_eq_on_vars [simp]:
+  "s\<^sub>1 = s\<^sub>2 on set (vars a) \<Longrightarrow> aval a s\<^sub>1 = aval a s\<^sub>2"
+  apply (induction a)
+  apply auto 
+  using atomVal_eq_if_eq_on_vars eq_on_subset
+  apply (metis sup.cobounded1 sup.cobounded2)+
+  done
+
+fun lvars :: "com \<Rightarrow> vname set" where
+"lvars SKIP = {}" |
+"lvars (x::=e) = {x}" |
+"lvars (c1;;c2) = lvars c1 \<union> lvars c2" |
+"lvars (IF b\<noteq>0 THEN c1 ELSE c2) = lvars c1 \<union> lvars c2" |
+"lvars (WHILE b\<noteq>0 DO c) = lvars c"
+
+instantiation com :: vars
+begin
+
+fun vars_com :: "com \<Rightarrow> vname list" where
+"vars SKIP = []" |
+"vars (x::=e) = x#vars e" |
+"vars (c1;;c2) = vars c1 @ vars c2" |
+"vars (IF b\<noteq>0 THEN c1 ELSE c2) = b # vars c1 @ vars c2" |
+"vars (WHILE b\<noteq>0 DO c) = b#vars c"
+
+instance ..
+
+end
+
+instantiation com :: subst
+begin
+
+fun subst_com :: "(vname \<Rightarrow> vname) \<Rightarrow> com \<Rightarrow> com" where
+"subst m SKIP = SKIP" |
+"subst m (x::=e) = (m x) ::= subst m e" |
+"subst m (c\<^sub>1;;c\<^sub>2) = subst m c\<^sub>1;; subst m c\<^sub>2" |
+"subst m (IF b\<noteq>0 THEN c\<^sub>1 ELSE c\<^sub>2) = IF m b\<noteq>0 THEN subst m c\<^sub>1 ELSE subst m c\<^sub>2" |
+"subst m (WHILE b\<noteq>0 DO c) = WHILE m b\<noteq>0 DO subst m c"
+
+instance
+proof (standard, goal_cases)
+  case (1 m c)
+  then show ?case by (induction c) auto
+qed
+
+end
+
+lemma atomVal_subst[simp]: "inj_on m (set (vars a)) \<Longrightarrow> atomVal (subst m a) s = (atomVal a (s o m))"
+  by (induction a) auto
+
+lemma aval_subst[simp]: "inj_on m (set (vars a)) \<Longrightarrow> aval (subst m a) s = aval a (s o m)"
+  by (induction a) (auto simp add: inj_on_Un)
+
+context BS_Generalized_Cost begin
+
+lemma var_unchanged: "(c,s) \<Rightarrow>\<^sub>G\<^bsup>z\<^esup> t \<Longrightarrow> v \<notin> set (vars c) \<Longrightarrow> s v = t v"
+  apply (induction c s z t  rule: big_step_tG_induct)
+  using BS_Generalized_Cost_axioms
+  apply simp
+  subgoal using BS_Generalized_Cost_axioms 
+    by simp
+  by simp+
+
+lemma fresh_var_changed: "(c,s) \<Rightarrow>\<^sub>G\<^bsup>z\<^esup> t \<Longrightarrow> v \<notin> set (vars c) \<Longrightarrow> (c,s(v:=y)) \<Rightarrow>\<^sub>G\<^bsup>g\<^esup> t' \<Longrightarrow> t' = t(v:=y)"
+proof (induction c s z t arbitrary: g t' rule: big_step_tG_induct)
+  case (1 s)
+  then show ?case 
+  using BS_Generalized_Cost_axioms by simp
+next
+  case (2 x a s)
+  then show ?case 
+  using BS_Generalized_Cost_axioms by auto
+qed auto
+
+lemma lvars_unchanged: "(c,s) \<Rightarrow>\<^sub>G\<^bsup>z\<^esup> t \<Longrightarrow> v \<notin> lvars c \<Longrightarrow> s v = t v"
+  apply (induction c s z t arbitrary:  rule: big_step_tG_induct)
+  using BS_Generalized_Cost_axioms by simp+
+
+lemma subst_costs:
+  "\<lbrakk>(subst m (x ::= a),s) \<Rightarrow>\<^sub>G\<^bsup> z \<^esup> t' \<rbrakk> \<Longrightarrow> z = assign_costs (subst m a) s"
+  unfolding eq_on_def by (auto simp:  aval_eq_if_eq_on_vars[unfolded eq_on_def])   
+
+
+lemma atom_Val_costs: 
+  "\<lbrakk> s = s' o m on S; set (vars a) \<subseteq> S; inj_on m S \<rbrakk>
+    \<Longrightarrow>  atomVal_cost (subst m a) s' = atomVal_cost a s" unfolding eq_on_def
+  apply (auto simp: subset_inj_on subsetD inj_on_contraD aval_eq_if_eq_on_vars[unfolded eq_on_def])
+  by (induction a)  auto
+
+lemma aexp_costs: 
+  "\<lbrakk> s = s' o m on S; set (vars a) \<subseteq> S; inj_on m S \<rbrakk>
+    \<Longrightarrow>  aexp_cost (subst m a) s' = aexp_cost a s"unfolding eq_on_def
+  apply (auto simp: subset_inj_on subsetD inj_on_contraD aval_eq_if_eq_on_vars[unfolded eq_on_def])
+  apply (induction a) apply auto
+  by (metis atom_Val_costs comp_def eq_onI)+
+
+lemma subst_costs_assign:
+  "\<lbrakk> s = s' o m on S; set (vars (x ::= a)) \<subseteq> S; inj_on m S \<rbrakk>
+    \<Longrightarrow>  assign_costs (subst m a) s' = assign_costs a s" unfolding eq_on_def
+  apply (auto simp: subset_inj_on subsetD inj_on_contraD aval_eq_if_eq_on_vars[unfolded eq_on_def])
+  apply (induction a) apply auto
+  by (metis atom_Val_costs comp_eq_dest_lhs eq_onI)+
+  term "(m x) ::= subst m a"
+
+lemma obtain_existing: 
+  assumes "\<exists>t'. P t'"
+  obtains t' where "P t'"
+  sledgehammer
+  using assms by auto
+
+lemma subst_sound':
+  "\<lbrakk> (c,s) \<Rightarrow>\<^sub>G\<^bsup>z\<^esup> t; s = s' o m on S; set (vars c) \<subseteq> S; inj_on m S \<rbrakk>
+    \<Longrightarrow> \<exists>t' z'. (subst m c,s') \<Rightarrow>\<^sub>G\<^bsup>z'\<^esup> t' \<and> t = t' o m on S"
+proof (induction c s z t arbitrary: s' rule: big_step_tG_induct)
+  case (1 s)
+  have "(subst m SKIP, s') \<Rightarrow>\<^sub>G\<^bsup> skip_costs s' \<^esup> s'"
+    by simp
+  then show ?case using "1.prems"(1) by auto
+next
+  case  (2 x a s) then show ?case unfolding eq_on_def
+    apply (auto simp: subset_inj_on subsetD inj_on_contraD aval_eq_if_eq_on_vars[unfolded eq_on_def])
+    apply (standard)+
+     apply (simp add: BS_Generalized_Cost_axioms)
+    apply (standard)+
+     apply (metis "2.prems"(1) aval_eq_if_eq_on_vars aval_subst eq_on_subset fun_upd_same inj_on_subset)
+    by (simp add: inj_on_contraD)
+next
+  case (3 c1 s1 C1 s2 c2 C2 s3 C3)
+  have "set (vars c1) \<subseteq> S" and "set (vars c2) \<subseteq> S" using \<open>set (vars (c1;; c2)) \<subseteq> S\<close> by auto
+  have "\<exists>s2' z'. (((subst m c1, s') \<Rightarrow>\<^sub>G\<^bsup> z' \<^esup> s2') \<and> s2 = s2' \<circ> m on S)"
+    using \<open>s1 = s' \<circ> m on S\<close>  \<open>inj_on m S\<close> \<open>set (vars c1) \<subseteq> S\<close> "3.IH"(1)[of s']
+    by blast
+  then obtain s2' z' where 1: "(subst m c1, s') \<Rightarrow>\<^sub>G\<^bsup> z' \<^esup> s2'" "s2 = s2' \<circ> m on S"    
+    by force
+  have "\<exists>t' z'. ((subst m c2, s2') \<Rightarrow>\<^sub>G\<^bsup> z' \<^esup> t' \<and> s3 = t' \<circ> m on S)"
+    using \<open>s2 = s2' \<circ> m on S\<close>  \<open>inj_on m S\<close> \<open>set (vars c2) \<subseteq> S\<close> "3.IH"(2)[of s2']
+    by blast
+ (* Works with WhileTrue; Esoteric*)
+  with Seq obtain s3' z'' where 2: "(subst m c2, s2')  \<Rightarrow>\<^sub>G\<^bsup> z'' \<^esup> s3'" "s3 = s3' \<circ> m on S" unfolding eq_on_def
+    by blast
+  let ?z''' = "z' + z''"
+  have "(subst m (c1;; c2), s') \<Rightarrow>\<^sub>G\<^bsup> ?z''' \<^esup> s3'"
+    using  1 2 Seq by auto
+  then show ?case unfolding eq_on_def using \<open>s3 = s3' \<circ> m on S\<close> by blast
+next
+  case (4 s b c1 C t C' c2)
+  have "set (vars c1) \<subseteq> S" and "set (vars c2) \<subseteq> S" using \<open>set (vars (IF b\<noteq>0 THEN c1 ELSE c2)) \<subseteq> S\<close> by auto
+  have "\<exists>s2' z'. (((subst m c1, s') \<Rightarrow>\<^sub>G\<^bsup> z' \<^esup> s2') \<and> t = s2' \<circ> m on S)"
+    using \<open>s = s' \<circ> m on S\<close>  \<open>inj_on m S\<close> \<open>set (vars c1) \<subseteq> S\<close> "4.IH"(1)[of s']
+    by blast
+  then obtain s2' z' where 1: "(subst m c1, s') \<Rightarrow>\<^sub>G\<^bsup> z' \<^esup> s2'" "t = s2' \<circ> m on S"    
+    by force
+  have "s'(m b) \<noteq> 0" using \<open>s b \<noteq> 0\<close> \<open>s = s' \<circ> m on S\<close>  \<open>set (vars (IF b\<noteq>0 THEN c1 ELSE c2)) \<subseteq> S\<close> unfolding eq_on_def by auto
+  have "(subst m (IF b\<noteq>0 THEN c1 ELSE c2), s') \<Rightarrow>\<^sub>G\<^bsup> z' + 1 \<^esup> s2'"
+    using 1 IfTrue \<open>s'(m b) \<noteq> 0\<close> by auto
+  then show ?case unfolding eq_on_def using \<open>t = s2' \<circ> m on S\<close> by blast
+next
+  case (5 s b c2 C t C' c1)
+  have "set (vars c1) \<subseteq> S" and "set (vars c2) \<subseteq> S" using \<open>set (vars (IF b\<noteq>0 THEN c1 ELSE c2)) \<subseteq> S\<close> by auto
+  have "\<exists>s2' z'. (((subst m c2, s') \<Rightarrow>\<^sub>G\<^bsup> z' \<^esup> s2') \<and> t = s2' \<circ> m on S)"
+    using \<open>s = s' \<circ> m on S\<close>  \<open>inj_on m S\<close> \<open>set (vars c2) \<subseteq> S\<close> "5.IH"(1)[of s']
+    by blast
+  then obtain s2' z' where 1: "(subst m c2, s') \<Rightarrow>\<^sub>G\<^bsup> z' \<^esup> s2'" "t = s2' \<circ> m on S"    
+    by force
+  have "s'(m b) = 0" using \<open>s b = 0\<close> \<open>s = s' \<circ> m on S\<close>  \<open>set (vars (IF b\<noteq>0 THEN c1 ELSE c2)) \<subseteq> S\<close> unfolding eq_on_def by auto
+  have "(subst m (IF b\<noteq>0 THEN c1 ELSE c2), s') \<Rightarrow>\<^sub>G\<^bsup> z' + 1 \<^esup> s2'"
+    using 1 IfFalse \<open>s'(m b) = 0\<close> by auto
+  then show ?case unfolding eq_on_def using \<open>t = s2' \<circ> m on S\<close> by blast
+next
+  case (6 s b c) 
+  have "s'(m b) = 0" using \<open>s b = 0\<close> \<open>s = s' \<circ> m on S\<close> \<open>set (vars (WHILE b\<noteq>0 DO c)) \<subseteq> S\<close> unfolding eq_on_def by auto
+  have "(subst m (WHILE b\<noteq>0 DO c), s') \<Rightarrow>\<^sub>G\<^bsup> while_exit_costs s' \<^esup> s'"
+    using \<open>s'(m b) = 0\<close> 
+    using big_step_tG.WhileFalse by auto
+  then show ?case 
+    using "6.prems"(1) by auto
+next
+  case (7 s1 b c C1 s2 C2 s3 C3)
+  have "set (vars c) \<subseteq> S" using \<open>set (vars (WHILE b\<noteq>0 DO c)) \<subseteq> S\<close> by auto
+  have "\<exists>s2' z'. (((subst m c, s') \<Rightarrow>\<^sub>G\<^bsup> z' \<^esup> s2') \<and> s2 = s2' \<circ> m on S)"
+    using \<open>s1 = s' \<circ> m on S\<close>  \<open>inj_on m S\<close> \<open>set (vars c) \<subseteq> S\<close>  "7.IH"(1)[of s']
+    by blast
+  then obtain s2' z' where 1: "(subst m c, s') \<Rightarrow>\<^sub>G\<^bsup> z' \<^esup> s2'" "s2 = s2' \<circ> m on S"    
+    by force
+  have "\<exists>t' z'. ((subst m (WHILE b\<noteq>0 DO c), s2') \<Rightarrow>\<^sub>G\<^bsup> z' \<^esup> t' \<and> s3 = t' \<circ> m on S)"
+    using \<open>s2 = s2' \<circ> m on S\<close>  \<open>inj_on m S\<close> \<open>set (vars (WHILE b\<noteq>0 DO c)) \<subseteq> S\<close> "7.IH"(2)[of s2']
+    by blast
+  with WhileTrue obtain s3' z'' where 2: "(subst m (WHILE b\<noteq>0 DO c), s2')  \<Rightarrow>\<^sub>G\<^bsup> z'' \<^esup> s3'" "s3 = s3' \<circ> m on S" unfolding eq_on_def
+    by blast
+  have "s'(m b) \<noteq> 0" using \<open>s1 b \<noteq> 0\<close> \<open>s1 = s' \<circ> m on S\<close> \<open>set (vars (WHILE b\<noteq>0 DO c)) \<subseteq> S\<close> unfolding eq_on_def by auto
+  have "((WHILE m b\<noteq>0 DO subst m c), s2')  \<Rightarrow>\<^sub>G\<^bsup> z'' \<^esup> s3'"
+    using \<open>(subst m (WHILE b\<noteq>0 DO c), s2')  \<Rightarrow>\<^sub>G\<^bsup> z'' \<^esup> s3'\<close> by auto
+  let ?z''' = "z' + z'' + 1"
+  have " (WHILE m b\<noteq>0 DO (subst m c), s') \<Rightarrow>\<^sub>G\<^bsup> ?z''' \<^esup> s3'"
+    using \<open>s'(m b) \<noteq> 0\<close> 1 \<open>((WHILE m b\<noteq>0 DO subst m c), s2')  \<Rightarrow>\<^sub>G\<^bsup> z'' \<^esup> s3'\<close>  WhileTrue by auto
+    then show ?case unfolding eq_on_def using \<open>s3 = s3' \<circ> m on S\<close> by force
+qed 
+
+
+(* TODO: Skip issue. Cost may still be different *)
+lemma subst_costs_unchanged:
+  "\<lbrakk> (c,s) \<Rightarrow>\<^sub>G\<^bsup>z\<^esup> t; s = s' o m on S; set (vars c) \<subseteq> S; inj_on m S \<rbrakk>
+    \<Longrightarrow> \<exists>t' . (subst m c,s') \<Rightarrow>\<^sub>G\<^bsup>z\<^esup> t'"
+proof (induction c s z t arbitrary: s' rule: big_step_tG_induct)
+  case (1 s)
+  then show ?case unfolding eq_on_def apply auto sorry
+next
+  case (2 x a s)
+  then show ?case unfolding eq_on_def
+    apply (auto simp: subset_inj_on subsetD inj_on_contraD aval_eq_if_eq_on_vars[unfolded eq_on_def])
+    by (metis "2.prems"(1) BS_Generalized_Cost.aexp_costs BS_Generalized_Cost_axioms Suc_eq_plus1 big_step_tG.Assign)
+next
+  case (3 c1 s1 C1 s2 c2 C2 s3 C3)
+  then show ?case unfolding eq_on_def
+    apply (auto simp: subset_inj_on subsetD inj_on_contraD aval_eq_if_eq_on_vars[unfolded eq_on_def])
+    by (metis (full_types) "3.IH"(1) "3.IH"(2) "3.prems"(1) local.bigstep_det local.compose_programs_1 subst_sound')
+next
+  case (4 s b c1 C t C' c2)
+  have "set (vars c1) \<subseteq> S" and "set (vars c2) \<subseteq> S" using \<open>set (vars (IF b\<noteq>0 THEN c1 ELSE c2)) \<subseteq> S\<close> by auto
+  have "\<exists>s2'. (((subst m c1, s') \<Rightarrow>\<^sub>G\<^bsup> C \<^esup> s2'))"
+    using \<open>s = s' \<circ> m on S\<close>  \<open>inj_on m S\<close> \<open>set (vars c1) \<subseteq> S\<close> "4.IH"(1)[of s']
+    by blast
+  then obtain s2'  where 1: "(subst m c1, s') \<Rightarrow>\<^sub>G\<^bsup> C \<^esup> s2'"   
+    by force
+  have "s'(m b) \<noteq> 0" using \<open>s b \<noteq> 0\<close> \<open>s = s' \<circ> m on S\<close>  \<open>set (vars (IF b\<noteq>0 THEN c1 ELSE c2)) \<subseteq> S\<close> unfolding eq_on_def by auto
+  have "(subst m (IF b\<noteq>0 THEN c1 ELSE c2), s') \<Rightarrow>\<^sub>G\<^bsup> C + 1 \<^esup> s2'"
+    using 1 IfTrue \<open>s'(m b) \<noteq> 0\<close> by auto
+  then show ?case unfolding eq_on_def 
+    using "4.hyps"(3) by blast
+next
+  case (5 s b c2 C t C' c1)
+  have "set (vars c1) \<subseteq> S" and "set (vars c2) \<subseteq> S" using \<open>set (vars (IF b\<noteq>0 THEN c1 ELSE c2)) \<subseteq> S\<close> by auto
+  have "\<exists>s2' . (((subst m c2, s') \<Rightarrow>\<^sub>G\<^bsup> C \<^esup> s2'))"
+    using \<open>s = s' \<circ> m on S\<close>  \<open>inj_on m S\<close> \<open>set (vars c2) \<subseteq> S\<close> "5.IH"(1)[of s']
+    by blast
+  then obtain s2' where 1: "(subst m c2, s') \<Rightarrow>\<^sub>G\<^bsup> C \<^esup> s2'"   
+    by force
+  have "s'(m b) = 0" using \<open>s b = 0\<close> \<open>s = s' \<circ> m on S\<close>  \<open>set (vars (IF b\<noteq>0 THEN c1 ELSE c2)) \<subseteq> S\<close> unfolding eq_on_def by auto
+  have "(subst m (IF b\<noteq>0 THEN c1 ELSE c2), s') \<Rightarrow>\<^sub>G\<^bsup> C + 1 \<^esup> s2'"
+    using 1 IfFalse \<open>s'(m b) = 0\<close> by auto
+  then show ?case unfolding eq_on_def 
+    using "5.hyps"(3) by blast
+next
+  case (6 s b c)
+  then show ?case sorry
+next
+  case (7 s1 b c C1 s2 C2 s3 C3)
+  have "set (vars c) \<subseteq> S" using \<open>set (vars (WHILE b\<noteq>0 DO c)) \<subseteq> S\<close> by auto
+  have "\<exists>s2'. (((subst m c, s') \<Rightarrow>\<^sub>G\<^bsup> C1 \<^esup> s2'))"
+    using \<open>s1 = s' \<circ> m on S\<close>  \<open>inj_on m S\<close> \<open>set (vars c) \<subseteq> S\<close>  "7.IH"(1)[of s']
+    by blast
+  then obtain s2' where 1: "(subst m c, s') \<Rightarrow>\<^sub>G\<^bsup> C1 \<^esup> s2'"    
+    by force
+  have \<open>s2 = s2' \<circ> m on S\<close> using subst_sound' big_step_t_cost_determ2 
+    by (metis "1" "7.hyps"(2) "7.prems"(1) "7.prems"(3) BS_Generalized_Cost.big_step_t_state_determ2 BS_Generalized_Cost_axioms \<open>set (vars c) \<subseteq> S\<close>)
+  have "\<exists>t' . ((subst m (WHILE b\<noteq>0 DO c), s2') \<Rightarrow>\<^sub>G\<^bsup> C2 \<^esup> t')"
+    using \<open>s2 = s2' \<circ> m on S\<close>  \<open>inj_on m S\<close> \<open>set (vars (WHILE b\<noteq>0 DO c)) \<subseteq> S\<close> "7.IH"(2)[of s2']
+    by blast
+  with WhileTrue obtain s3' where 2: "(subst m (WHILE b\<noteq>0 DO c), s2')  \<Rightarrow>\<^sub>G\<^bsup> C2 \<^esup> s3'"  unfolding eq_on_def
+    by blast
+  have "s'(m b) \<noteq> 0" using \<open>s1 b \<noteq> 0\<close> \<open>s1 = s' \<circ> m on S\<close> \<open>set (vars (WHILE b\<noteq>0 DO c)) \<subseteq> S\<close> unfolding eq_on_def by auto
+  have "((WHILE m b\<noteq>0 DO subst m c), s2')  \<Rightarrow>\<^sub>G\<^bsup> C2 \<^esup> s3'"
+    using \<open>(subst m (WHILE b\<noteq>0 DO c), s2')  \<Rightarrow>\<^sub>G\<^bsup> C2 \<^esup> s3'\<close> by auto
+  let ?z''' = "C1 + C2 + 1"
+  have " (WHILE m b\<noteq>0 DO (subst m c), s') \<Rightarrow>\<^sub>G\<^bsup> ?z''' \<^esup> s3'"
+    using \<open>s'(m b) \<noteq> 0\<close> 1 \<open>((WHILE m b\<noteq>0 DO subst m c), s2')  \<Rightarrow>\<^sub>G\<^bsup> C2 \<^esup> s3'\<close>  WhileTrue by auto
+    then show ?case unfolding eq_on_def using \<open>C3 = C1 + C2 + 1\<close> by auto
+qed
+
+lemma subst_sound:
+  "\<lbrakk> (c,s) \<Rightarrow>\<^sub>G\<^bsup>z\<^esup> t; s = s' o m on S; set (vars c) \<subseteq> S; inj_on m S \<rbrakk>
+    \<Longrightarrow> \<exists>t' z' . (subst m c,s') \<Rightarrow>\<^sub>G\<^bsup>z'\<^esup> t' \<and> t = t' o m on S"
+  using subst_sound' subst_costs_unchanged by (metis big_step_t_state_determ2)
+
+lemma subst_complete':
+  "\<lbrakk> (subst m c,s') \<Rightarrow>\<^sub>G\<^bsup>z\<^esup> t'; s = s' o m on S; set (vars c) \<subseteq> S; inj_on m S \<rbrakk>
+    \<Longrightarrow> \<exists>t z'. (c,s) \<Rightarrow>\<^sub>G\<^bsup>z'\<^esup> t \<and> t = t' o m on S"
+proof (induction "subst m c" s' z t' arbitrary: c s rule: big_step_tG_induct)
+  case (1 s)
+  then show ?case apply (cases c) by auto 
+next
+  case (2 x a  s' c s)
+  then obtain x' a' where defs: "c = x' ::= a'" "x = m x'" "a = subst m a'" by (cases c) auto
+  moreover have "(x' ::= a',s) \<Rightarrow>\<^sub>G\<^bsup>assign_costs a s' \<^esup> s(x' := aval a' s)" apply auto
+    by (metis "2.prems"(1) "2.prems"(2) "2.prems"(3) Suc_eq_plus1 calculation(1) calculation(3) local.ASSnot subst_costs_assign)
+  moreover have "s(x' := aval a' s) = s'(x := aval a s') \<circ> m on S"
+    (* Error about online proof reconstruction *)
+    by (smt (verit) "2.hyps" "2.prems"(1) "2.prems"(2) "2.prems"(3) big_step_tG.Assign big_step_t_state_determ2 calculation(1) subst_sound') 
+  ultimately show ?case 
+    by metis
+next
+  case (3 c\<^sub>1 s\<^sub>1 x s\<^sub>2 c\<^sub>2 y s\<^sub>3 z c s\<^sub>1')
+  then show ?case using 3 apply (cases c) apply auto
+    by (metis (no_types, lifting) big_step_tG.Seq)
+next
+  case (4 s b c\<^sub>1 x t z c\<^sub>2 c s')
+  then show ?case apply (cases c) apply auto
+(* Timed out, trusting that false case works similarly *)
+    by (smt (verit) "4.hyps"(1) "4.hyps"(4) big_step_tG.IfTrue comp_apply eq_onE)
+next
+  case (5 s b c2 C t C' c1)
+  then show ?case apply (cases c) apply auto
+    by (smt (verit) "5.hyps"(1) "5.hyps"(4) big_step_tG.IfFalse comp_apply eq_onE)
+next
+  case (6 s b c\<^sub>1 c s')
+  then show ?case apply (cases c) apply auto 
+    by (metis big_step_tG.WhileFalse comp_def eq_onD)
+next
+  case (7 s\<^sub>1 b c\<^sub>1 x s\<^sub>2 y s\<^sub>3 z c s\<^sub>1')
+  then obtain c\<^sub>1' b' where [simp]: "c = WHILE b'\<noteq>0 DO c\<^sub>1'" "m b' = b" "c\<^sub>1 = subst m c\<^sub>1'" by (cases c) auto
+  with 7 have "set (vars c\<^sub>1') \<subseteq> S" by auto 
+  with "7.hyps"(3)[OF _ "7.prems"(1) this "7.prems"(3)] obtain s\<^sub>2' z' where
+    1: "(c\<^sub>1', s\<^sub>1') \<Rightarrow>\<^sub>G\<^bsup> z' \<^esup> s\<^sub>2'" "s\<^sub>2' = s\<^sub>2 \<circ> m on S" by auto 
+  with "7.hyps"(5)[OF _ this(2) "7.prems"(2) "7.prems"(3)] obtain s\<^sub>3' z'' where
+    2: "(WHILE b'\<noteq>0 DO c\<^sub>1', s\<^sub>2')  \<Rightarrow>\<^sub>G\<^bsup> z'' \<^esup> s\<^sub>3'" "s\<^sub>3' = s\<^sub>3 \<circ> m on S" by auto
+  from 1 2 "7.hyps"(1,6) "7.prems"(1,2) have
+    "(WHILE b'\<noteq>0 DO c\<^sub>1', s\<^sub>1')  \<Rightarrow>\<^sub>G\<^bsup> z' + z'' + 1 \<^esup> s\<^sub>3'" "s\<^sub>3' = s\<^sub>3 \<circ> m on S" unfolding eq_on_def using Seq_tE_While_init While_tE apply auto
+    by (metis "7.hyps"(1) Suc_eq_plus1 \<open>m b' = b\<close> big_step_tG.WhileTrue)
+  thus ?case by auto
+qed
+
+lemma subst_complete:
+  "\<lbrakk> (subst m c,s') \<Rightarrow>\<^sub>G\<^bsup>z\<^esup> t'; s = s' o m on S; set (vars c) \<subseteq> S; inj_on m S \<rbrakk>
+    \<Longrightarrow> \<exists>t . (c,s) \<Rightarrow>\<^sub>G\<^bsup>z\<^esup> t \<and> t = t' o m on S"
+  using subst_complete' subst_costs_unchanged  by (metis local.bigstep_det)
+
+lemma noninterference': 
+  "(c,s) \<Rightarrow>\<^sub>G\<^bsup> x \<^esup> t \<Longrightarrow> set (vars c) \<subseteq> S \<Longrightarrow> s = s' on S \<Longrightarrow> \<exists>t' z'. (c,s') \<Rightarrow>\<^sub>G\<^bsup> z' \<^esup> t' \<and> t = t' on S"
+proof (induction c s x t arbitrary: s' rule: big_step_tG_induct)
+  case (1 s)
+  then show ?case by auto 
+next
+  case (2 x a s)
+  then show ?case unfolding eq_on_def
+    apply (auto simp: subset_inj_on subsetD inj_on_contraD aval_eq_if_eq_on_vars[unfolded eq_on_def])
+    by (metis "2.prems"(2) aval_eq_if_eq_on_vars big_step_tG.Assign eq_on_subset fun_upd_other fun_upd_same)
+next
+  case (3 c1 s1 C1 s2 c2 C2 s3 C3)
+  then show ?case  unfolding eq_on_def
+    apply (auto simp: subset_inj_on subsetD inj_on_contraD aval_eq_if_eq_on_vars[unfolded eq_on_def])
+    sorry
+next
+  case (4 s b c1 C t C' c2)
+  then show ?case sorry
+next
+  case (5 s b c2 C t C' c1)
+  then show ?case sorry
+next
+  case (6 s b c)
+  then show ?case sorry
+next
+  case (7 s1 b c C1 s2 C2 s3 C3)
+  then show ?case sorry
+qed
+  case (Assign x a s)
+  then show ?case 
+    using aval_eq_if_eq_on_vars big_step_t.Assign eq_on_def eq_on_subset fun_upd_apply set_subset_Cons vars_com.simps(2) by fastforce
+next
+  case (WhileTrue s1 b c x s2 y s3 z)
+  then show ?case apply auto
+    by (metis (mono_tags, lifting) WhileTrue.hyps(1) WhileTrue.hyps(4) big_step_t.WhileTrue eq_onE)
+qed fastforce+
+
+
+end
